Ch 10 + control

rocq/control/syntax.sig
@@ -1,0 +1,58 @@
+bool : Type
+nat  : Type
+list : Functor
+
+Val(var) : Type
+Tm       : Type
+Frame    : Type
+
+
+-- Values
+unit   : Val
+zero   : Val
+succ   : Val -> Val
+prod   : Val -> Val -> Val
+inj    : bool -> Val -> Val
+abs    : (bind Val in Tm) -> Val
+rec    : (bind Val in Val) -> Val
+fold   : Val -> Val
+
+-- continuation value, a saved stack
+cont   : "list"(Frame) -> Val
+-- effect constructors
+eff    : nat -> Val
+
+-- Terms / Computations
+ret     : Val -> Tm
+let_    : Tm -> (bind Val in Tm) -> Tm
+ifz     : Val -> Tm -> (bind Val in Tm) -> Tm
+prj     : bool -> Val -> Tm
+case    : Val -> (bind Val in Tm) -> (bind Val in Tm) -> Tm
+app     : Val -> Val -> Tm
+unfold  : Val -> Tm
+
+-- exceptions
+raise   : Val -> Tm
+try     : Tm -> (bind Val in Tm) -> Tm
+
+-- continuations
+throw   : Val -> Val -> Tm
+letcc   : (bind Val in Tm) -> Tm
+
+-- effect handlers
+perform  : Val -> Tm
+handle   : Tm -> (bind Val in Tm) -> nat -> (bind Val in Tm) -> Tm
+continue : Val -> Val -> Tm
+
+-- frames
+f_try    : (bind Val in Tm) -> Frame
+f_let    : (bind Val in Tm) -> Frame
+f_handle : (bind Val in Tm) -> nat -> (bind Val in Tm) -> Frame
+
+
+-- HOMEWORK
+v_nil       : Val
+v_cons      : Val -> Val -> Val
+throw_e     : Val -> Tm -> Tm
+exit        : Val -> Tm 
+discontinue : Val -> Val -> Tm
