rocq/control/typesyntax.sig
@@ -1,0 +1,15 @@
+-- Types
+Ty     : Type
+Unit   : Ty
+Void   : Ty
+Nat    : Ty
+Prod   : Ty -> Ty -> Ty
+Sum    : Ty -> Ty -> Ty
+Arr    : Ty -> Ty -> Ty
+Mu     : (bind Ty in Ty) -> Ty
+Cont   : Ty -> Ty
+Eff    : Ty -> Ty
+DeCont : Ty -> Ty -> Ty
+
+-- HOMEWORK
+List   : Ty -> Ty
