rocq/control/syntax.v
@@ -1,0 +1,2310 @@
+Require Import core fintype.
+
+Require Import Setoid Morphisms Relation_Definitions.
+
+
+Module Core.
+
+Inductive Val (n_Val : nat) : Type :=
+  | var : fin n_Val -> Val n_Val
+  | unit : Val n_Val
+  | zero : Val n_Val
+  | succ : Val n_Val -> Val n_Val
+  | prod : Val n_Val -> Val n_Val -> Val n_Val
+  | inj : bool -> Val n_Val -> Val n_Val
+  | abs : Tm (S n_Val) -> Val n_Val
+  | rec : Val (S n_Val) -> Val n_Val
+  | fold : Val n_Val -> Val n_Val
+  | cont : list (Frame n_Val) -> Val n_Val
+  | eff : nat -> Val n_Val
+  | v_nil : Val n_Val
+  | v_cons : Val n_Val -> Val n_Val -> Val n_Val
+with Tm (n_Val : nat) : Type :=
+  | ret : Val n_Val -> Tm n_Val
+  | let_ : Tm n_Val -> Tm (S n_Val) -> Tm n_Val
+  | ifz : Val n_Val -> Tm n_Val -> Tm (S n_Val) -> Tm n_Val
+  | prj : bool -> Val n_Val -> Tm n_Val
+  | case : Val n_Val -> Tm (S n_Val) -> Tm (S n_Val) -> Tm n_Val
+  | app : Val n_Val -> Val n_Val -> Tm n_Val
+  | unfold : Val n_Val -> Tm n_Val
+  | raise : Val n_Val -> Tm n_Val
+  | try : Tm n_Val -> Tm (S n_Val) -> Tm n_Val
+  | throw : Val n_Val -> Val n_Val -> Tm n_Val
+  | letcc : Tm (S n_Val) -> Tm n_Val
+  | perform : Val n_Val -> Tm n_Val
+  | handle : Tm n_Val -> Tm (S n_Val) -> nat -> Tm (S n_Val) -> Tm n_Val
+  | continue : Val n_Val -> Val n_Val -> Tm n_Val
+  | throw_e : Val n_Val -> Tm n_Val -> Tm n_Val
+  | exit : Val n_Val -> Tm n_Val
+  | discontinue : Val n_Val -> Val n_Val -> Tm n_Val
+with Frame (n_Val : nat) : Type :=
+  | f_try : Tm (S n_Val) -> Frame n_Val
+  | f_let : Tm (S n_Val) -> Frame n_Val
+  | f_handle : Tm (S n_Val) -> nat -> Tm (S n_Val) -> Frame n_Val.
+
+Lemma congr_unit {m_Val : nat} : unit m_Val = unit m_Val.
+Proof.
+exact (eq_refl).
+Qed.
+
+Lemma congr_zero {m_Val : nat} : zero m_Val = zero m_Val.
+Proof.
+exact (eq_refl).
+Qed.
+
+Lemma congr_succ {m_Val : nat} {s0 : Val m_Val} {t0 : Val m_Val}
+  (H0 : s0 = t0) : succ m_Val s0 = succ m_Val t0.
+Proof.
+exact (eq_trans eq_refl (ap (fun x => succ m_Val x) H0)).
+Qed.
+
+Lemma congr_prod {m_Val : nat} {s0 : Val m_Val} {s1 : Val m_Val}
+  {t0 : Val m_Val} {t1 : Val m_Val} (H0 : s0 = t0) (H1 : s1 = t1) :
+  prod m_Val s0 s1 = prod m_Val t0 t1.
+Proof.
+exact (eq_trans (eq_trans eq_refl (ap (fun x => prod m_Val x s1) H0))
+         (ap (fun x => prod m_Val t0 x) H1)).
+Qed.
+
+Lemma congr_inj {m_Val : nat} {s0 : bool} {s1 : Val m_Val} {t0 : bool}
+  {t1 : Val m_Val} (H0 : s0 = t0) (H1 : s1 = t1) :
+  inj m_Val s0 s1 = inj m_Val t0 t1.
+Proof.
+exact (eq_trans (eq_trans eq_refl (ap (fun x => inj m_Val x s1) H0))
+         (ap (fun x => inj m_Val t0 x) H1)).
+Qed.
+
+Lemma congr_abs {m_Val : nat} {s0 : Tm (S m_Val)} {t0 : Tm (S m_Val)}
+  (H0 : s0 = t0) : abs m_Val s0 = abs m_Val t0.
+Proof.
+exact (eq_trans eq_refl (ap (fun x => abs m_Val x) H0)).
+Qed.
+
+Lemma congr_rec {m_Val : nat} {s0 : Val (S m_Val)} {t0 : Val (S m_Val)}
+  (H0 : s0 = t0) : rec m_Val s0 = rec m_Val t0.
+Proof.
+exact (eq_trans eq_refl (ap (fun x => rec m_Val x) H0)).
+Qed.
+
+Lemma congr_fold {m_Val : nat} {s0 : Val m_Val} {t0 : Val m_Val}
+  (H0 : s0 = t0) : fold m_Val s0 = fold m_Val t0.
+Proof.
+exact (eq_trans eq_refl (ap (fun x => fold m_Val x) H0)).
+Qed.
+
+Lemma congr_cont {m_Val : nat} {s0 : list (Frame m_Val)}
+  {t0 : list (Frame m_Val)} (H0 : s0 = t0) : cont m_Val s0 = cont m_Val t0.
+Proof.
+exact (eq_trans eq_refl (ap (fun x => cont m_Val x) H0)).
+Qed.
+
+Lemma congr_eff {m_Val : nat} {s0 : nat} {t0 : nat} (H0 : s0 = t0) :
+  eff m_Val s0 = eff m_Val t0.
+Proof.
+exact (eq_trans eq_refl (ap (fun x => eff m_Val x) H0)).
+Qed.
+
+Lemma congr_v_nil {m_Val : nat} : v_nil m_Val = v_nil m_Val.
+Proof.
+exact (eq_refl).
+Qed.
+
+Lemma congr_v_cons {m_Val : nat} {s0 : Val m_Val} {s1 : Val m_Val}
+  {t0 : Val m_Val} {t1 : Val m_Val} (H0 : s0 = t0) (H1 : s1 = t1) :
+  v_cons m_Val s0 s1 = v_cons m_Val t0 t1.
+Proof.
+exact (eq_trans (eq_trans eq_refl (ap (fun x => v_cons m_Val x s1) H0))
+         (ap (fun x => v_cons m_Val t0 x) H1)).
+Qed.
+
+Lemma congr_ret {m_Val : nat} {s0 : Val m_Val} {t0 : Val m_Val}
+  (H0 : s0 = t0) : ret m_Val s0 = ret m_Val t0.
+Proof.
+exact (eq_trans eq_refl (ap (fun x => ret m_Val x) H0)).
+Qed.
+
+Lemma congr_let_ {m_Val : nat} {s0 : Tm m_Val} {s1 : Tm (S m_Val)}
+  {t0 : Tm m_Val} {t1 : Tm (S m_Val)} (H0 : s0 = t0) (H1 : s1 = t1) :
+  let_ m_Val s0 s1 = let_ m_Val t0 t1.
+Proof.
+exact (eq_trans (eq_trans eq_refl (ap (fun x => let_ m_Val x s1) H0))
+         (ap (fun x => let_ m_Val t0 x) H1)).
+Qed.
+
+Lemma congr_ifz {m_Val : nat} {s0 : Val m_Val} {s1 : Tm m_Val}
+  {s2 : Tm (S m_Val)} {t0 : Val m_Val} {t1 : Tm m_Val} {t2 : Tm (S m_Val)}
+  (H0 : s0 = t0) (H1 : s1 = t1) (H2 : s2 = t2) :
+  ifz m_Val s0 s1 s2 = ifz m_Val t0 t1 t2.
+Proof.
+exact (eq_trans
+         (eq_trans (eq_trans eq_refl (ap (fun x => ifz m_Val x s1 s2) H0))
+            (ap (fun x => ifz m_Val t0 x s2) H1))
+         (ap (fun x => ifz m_Val t0 t1 x) H2)).
+Qed.
+
+Lemma congr_prj {m_Val : nat} {s0 : bool} {s1 : Val m_Val} {t0 : bool}
+  {t1 : Val m_Val} (H0 : s0 = t0) (H1 : s1 = t1) :
+  prj m_Val s0 s1 = prj m_Val t0 t1.
+Proof.
+exact (eq_trans (eq_trans eq_refl (ap (fun x => prj m_Val x s1) H0))
+         (ap (fun x => prj m_Val t0 x) H1)).
+Qed.
+
+Lemma congr_case {m_Val : nat} {s0 : Val m_Val} {s1 : Tm (S m_Val)}
+  {s2 : Tm (S m_Val)} {t0 : Val m_Val} {t1 : Tm (S m_Val)}
+  {t2 : Tm (S m_Val)} (H0 : s0 = t0) (H1 : s1 = t1) (H2 : s2 = t2) :
+  case m_Val s0 s1 s2 = case m_Val t0 t1 t2.
+Proof.
+exact (eq_trans
+         (eq_trans (eq_trans eq_refl (ap (fun x => case m_Val x s1 s2) H0))
+            (ap (fun x => case m_Val t0 x s2) H1))
+         (ap (fun x => case m_Val t0 t1 x) H2)).
+Qed.
+
+Lemma congr_app {m_Val : nat} {s0 : Val m_Val} {s1 : Val m_Val}
+  {t0 : Val m_Val} {t1 : Val m_Val} (H0 : s0 = t0) (H1 : s1 = t1) :
+  app m_Val s0 s1 = app m_Val t0 t1.
+Proof.
+exact (eq_trans (eq_trans eq_refl (ap (fun x => app m_Val x s1) H0))
+         (ap (fun x => app m_Val t0 x) H1)).
+Qed.
+
+Lemma congr_unfold {m_Val : nat} {s0 : Val m_Val} {t0 : Val m_Val}
+  (H0 : s0 = t0) : unfold m_Val s0 = unfold m_Val t0.
+Proof.
+exact (eq_trans eq_refl (ap (fun x => unfold m_Val x) H0)).
+Qed.
+
+Lemma congr_raise {m_Val : nat} {s0 : Val m_Val} {t0 : Val m_Val}
+  (H0 : s0 = t0) : raise m_Val s0 = raise m_Val t0.
+Proof.
+exact (eq_trans eq_refl (ap (fun x => raise m_Val x) H0)).
+Qed.
+
+Lemma congr_try {m_Val : nat} {s0 : Tm m_Val} {s1 : Tm (S m_Val)}
+  {t0 : Tm m_Val} {t1 : Tm (S m_Val)} (H0 : s0 = t0) (H1 : s1 = t1) :
+  try m_Val s0 s1 = try m_Val t0 t1.
+Proof.
+exact (eq_trans (eq_trans eq_refl (ap (fun x => try m_Val x s1) H0))
+         (ap (fun x => try m_Val t0 x) H1)).
+Qed.
+
+Lemma congr_throw {m_Val : nat} {s0 : Val m_Val} {s1 : Val m_Val}
+  {t0 : Val m_Val} {t1 : Val m_Val} (H0 : s0 = t0) (H1 : s1 = t1) :
+  throw m_Val s0 s1 = throw m_Val t0 t1.
+Proof.
+exact (eq_trans (eq_trans eq_refl (ap (fun x => throw m_Val x s1) H0))
+         (ap (fun x => throw m_Val t0 x) H1)).
+Qed.
+
+Lemma congr_letcc {m_Val : nat} {s0 : Tm (S m_Val)} {t0 : Tm (S m_Val)}
+  (H0 : s0 = t0) : letcc m_Val s0 = letcc m_Val t0.
+Proof.
+exact (eq_trans eq_refl (ap (fun x => letcc m_Val x) H0)).
+Qed.
+
+Lemma congr_perform {m_Val : nat} {s0 : Val m_Val} {t0 : Val m_Val}
+  (H0 : s0 = t0) : perform m_Val s0 = perform m_Val t0.
+Proof.
+exact (eq_trans eq_refl (ap (fun x => perform m_Val x) H0)).
+Qed.
+
+Lemma congr_handle {m_Val : nat} {s0 : Tm m_Val} {s1 : Tm (S m_Val)}
+  {s2 : nat} {s3 : Tm (S m_Val)} {t0 : Tm m_Val} {t1 : Tm (S m_Val)}
+  {t2 : nat} {t3 : Tm (S m_Val)} (H0 : s0 = t0) (H1 : s1 = t1) (H2 : s2 = t2)
+  (H3 : s3 = t3) : handle m_Val s0 s1 s2 s3 = handle m_Val t0 t1 t2 t3.
+Proof.
+exact (eq_trans
+         (eq_trans
+            (eq_trans
+               (eq_trans eq_refl (ap (fun x => handle m_Val x s1 s2 s3) H0))
+               (ap (fun x => handle m_Val t0 x s2 s3) H1))
+            (ap (fun x => handle m_Val t0 t1 x s3) H2))
+         (ap (fun x => handle m_Val t0 t1 t2 x) H3)).
+Qed.
+
+Lemma congr_continue {m_Val : nat} {s0 : Val m_Val} {s1 : Val m_Val}
+  {t0 : Val m_Val} {t1 : Val m_Val} (H0 : s0 = t0) (H1 : s1 = t1) :
+  continue m_Val s0 s1 = continue m_Val t0 t1.
+Proof.
+exact (eq_trans (eq_trans eq_refl (ap (fun x => continue m_Val x s1) H0))
+         (ap (fun x => continue m_Val t0 x) H1)).
+Qed.
+
+Lemma congr_throw_e {m_Val : nat} {s0 : Val m_Val} {s1 : Tm m_Val}
+  {t0 : Val m_Val} {t1 : Tm m_Val} (H0 : s0 = t0) (H1 : s1 = t1) :
+  throw_e m_Val s0 s1 = throw_e m_Val t0 t1.
+Proof.
+exact (eq_trans (eq_trans eq_refl (ap (fun x => throw_e m_Val x s1) H0))
+         (ap (fun x => throw_e m_Val t0 x) H1)).
+Qed.
+
+Lemma congr_exit {m_Val : nat} {s0 : Val m_Val} {t0 : Val m_Val}
+  (H0 : s0 = t0) : exit m_Val s0 = exit m_Val t0.
+Proof.
+exact (eq_trans eq_refl (ap (fun x => exit m_Val x) H0)).
+Qed.
+
+Lemma congr_discontinue {m_Val : nat} {s0 : Val m_Val} {s1 : Val m_Val}
+  {t0 : Val m_Val} {t1 : Val m_Val} (H0 : s0 = t0) (H1 : s1 = t1) :
+  discontinue m_Val s0 s1 = discontinue m_Val t0 t1.
+Proof.
+exact (eq_trans (eq_trans eq_refl (ap (fun x => discontinue m_Val x s1) H0))
+         (ap (fun x => discontinue m_Val t0 x) H1)).
+Qed.
+
+Lemma congr_f_try {m_Val : nat} {s0 : Tm (S m_Val)} {t0 : Tm (S m_Val)}
+  (H0 : s0 = t0) : f_try m_Val s0 = f_try m_Val t0.
+Proof.
+exact (eq_trans eq_refl (ap (fun x => f_try m_Val x) H0)).
+Qed.
+
+Lemma congr_f_let {m_Val : nat} {s0 : Tm (S m_Val)} {t0 : Tm (S m_Val)}
+  (H0 : s0 = t0) : f_let m_Val s0 = f_let m_Val t0.
+Proof.
+exact (eq_trans eq_refl (ap (fun x => f_let m_Val x) H0)).
+Qed.
+
+Lemma congr_f_handle {m_Val : nat} {s0 : Tm (S m_Val)} {s1 : nat}
+  {s2 : Tm (S m_Val)} {t0 : Tm (S m_Val)} {t1 : nat} {t2 : Tm (S m_Val)}
+  (H0 : s0 = t0) (H1 : s1 = t1) (H2 : s2 = t2) :
+  f_handle m_Val s0 s1 s2 = f_handle m_Val t0 t1 t2.
+Proof.
+exact (eq_trans
+         (eq_trans
+            (eq_trans eq_refl (ap (fun x => f_handle m_Val x s1 s2) H0))
+            (ap (fun x => f_handle m_Val t0 x s2) H1))
+         (ap (fun x => f_handle m_Val t0 t1 x) H2)).
+Qed.
+
+Lemma upRen_Val_Val {m : nat} {n : nat} (xi : fin m -> fin n) :
+  fin (S m) -> fin (S n).
+Proof.
+exact (up_ren xi).
+Defined.
+
+Lemma upRen_list_Val_Val (p : nat) {m : nat} {n : nat} (xi : fin m -> fin n)
+  : fin (plus p m) -> fin (plus p n).
+Proof.
+exact (upRen_p p xi).
+Defined.
+
+Fixpoint ren_Val {m_Val : nat} {n_Val : nat}
+(xi_Val : fin m_Val -> fin n_Val) (s : Val m_Val) {struct s} : Val n_Val :=
+  match s with
+  | var _ s0 => var n_Val (xi_Val s0)
+  | unit _ => unit n_Val
+  | zero _ => zero n_Val
+  | succ _ s0 => succ n_Val (ren_Val xi_Val s0)
+  | prod _ s0 s1 => prod n_Val (ren_Val xi_Val s0) (ren_Val xi_Val s1)
+  | inj _ s0 s1 => inj n_Val s0 (ren_Val xi_Val s1)
+  | abs _ s0 => abs n_Val (ren_Tm (upRen_Val_Val xi_Val) s0)
+  | rec _ s0 => rec n_Val (ren_Val (upRen_Val_Val xi_Val) s0)
+  | fold _ s0 => fold n_Val (ren_Val xi_Val s0)
+  | cont _ s0 => cont n_Val (list_map (ren_Frame xi_Val) s0)
+  | eff _ s0 => eff n_Val s0
+  | v_nil _ => v_nil n_Val
+  | v_cons _ s0 s1 => v_cons n_Val (ren_Val xi_Val s0) (ren_Val xi_Val s1)
+  end
+with ren_Tm {m_Val : nat} {n_Val : nat} (xi_Val : fin m_Val -> fin n_Val)
+(s : Tm m_Val) {struct s} : Tm n_Val :=
+  match s with
+  | ret _ s0 => ret n_Val (ren_Val xi_Val s0)
+  | let_ _ s0 s1 =>
+      let_ n_Val (ren_Tm xi_Val s0) (ren_Tm (upRen_Val_Val xi_Val) s1)
+  | ifz _ s0 s1 s2 =>
+      ifz n_Val (ren_Val xi_Val s0) (ren_Tm xi_Val s1)
+        (ren_Tm (upRen_Val_Val xi_Val) s2)
+  | prj _ s0 s1 => prj n_Val s0 (ren_Val xi_Val s1)
+  | case _ s0 s1 s2 =>
+      case n_Val (ren_Val xi_Val s0) (ren_Tm (upRen_Val_Val xi_Val) s1)
+        (ren_Tm (upRen_Val_Val xi_Val) s2)
+  | app _ s0 s1 => app n_Val (ren_Val xi_Val s0) (ren_Val xi_Val s1)
+  | unfold _ s0 => unfold n_Val (ren_Val xi_Val s0)
+  | raise _ s0 => raise n_Val (ren_Val xi_Val s0)
+  | try _ s0 s1 =>
+      try n_Val (ren_Tm xi_Val s0) (ren_Tm (upRen_Val_Val xi_Val) s1)
+  | throw _ s0 s1 => throw n_Val (ren_Val xi_Val s0) (ren_Val xi_Val s1)
+  | letcc _ s0 => letcc n_Val (ren_Tm (upRen_Val_Val xi_Val) s0)
+  | perform _ s0 => perform n_Val (ren_Val xi_Val s0)
+  | handle _ s0 s1 s2 s3 =>
+      handle n_Val (ren_Tm xi_Val s0) (ren_Tm (upRen_Val_Val xi_Val) s1) s2
+        (ren_Tm (upRen_Val_Val xi_Val) s3)
+  | continue _ s0 s1 =>
+      continue n_Val (ren_Val xi_Val s0) (ren_Val xi_Val s1)
+  | throw_e _ s0 s1 => throw_e n_Val (ren_Val xi_Val s0) (ren_Tm xi_Val s1)
+  | exit _ s0 => exit n_Val (ren_Val xi_Val s0)
+  | discontinue _ s0 s1 =>
+      discontinue n_Val (ren_Val xi_Val s0) (ren_Val xi_Val s1)
+  end
+with ren_Frame {m_Val : nat} {n_Val : nat} (xi_Val : fin m_Val -> fin n_Val)
+(s : Frame m_Val) {struct s} : Frame n_Val :=
+  match s with
+  | f_try _ s0 => f_try n_Val (ren_Tm (upRen_Val_Val xi_Val) s0)
+  | f_let _ s0 => f_let n_Val (ren_Tm (upRen_Val_Val xi_Val) s0)
+  | f_handle _ s0 s1 s2 =>
+      f_handle n_Val (ren_Tm (upRen_Val_Val xi_Val) s0) s1
+        (ren_Tm (upRen_Val_Val xi_Val) s2)
+  end.
+
+Lemma up_Val_Val {m : nat} {n_Val : nat} (sigma : fin m -> Val n_Val) :
+  fin (S m) -> Val (S n_Val).
+Proof.
+exact (scons (var (S n_Val) var_zero) (funcomp (ren_Val shift) sigma)).
+Defined.
+
+Lemma up_list_Val_Val (p : nat) {m : nat} {n_Val : nat}
+  (sigma : fin m -> Val n_Val) : fin (plus p m) -> Val (plus p n_Val).
+Proof.
+exact (scons_p p (funcomp (var (plus p n_Val)) (zero_p p))
+         (funcomp (ren_Val (shift_p p)) sigma)).
+Defined.
+
+Fixpoint subst_Val {m_Val : nat} {n_Val : nat}
+(sigma_Val : fin m_Val -> Val n_Val) (s : Val m_Val) {struct s} : Val n_Val
+:=
+  match s with
+  | var _ s0 => sigma_Val s0
+  | unit _ => unit n_Val
+  | zero _ => zero n_Val
+  | succ _ s0 => succ n_Val (subst_Val sigma_Val s0)
+  | prod _ s0 s1 =>
+      prod n_Val (subst_Val sigma_Val s0) (subst_Val sigma_Val s1)
+  | inj _ s0 s1 => inj n_Val s0 (subst_Val sigma_Val s1)
+  | abs _ s0 => abs n_Val (subst_Tm (up_Val_Val sigma_Val) s0)
+  | rec _ s0 => rec n_Val (subst_Val (up_Val_Val sigma_Val) s0)
+  | fold _ s0 => fold n_Val (subst_Val sigma_Val s0)
+  | cont _ s0 => cont n_Val (list_map (subst_Frame sigma_Val) s0)
+  | eff _ s0 => eff n_Val s0
+  | v_nil _ => v_nil n_Val
+  | v_cons _ s0 s1 =>
+      v_cons n_Val (subst_Val sigma_Val s0) (subst_Val sigma_Val s1)
+  end
+with subst_Tm {m_Val : nat} {n_Val : nat}
+(sigma_Val : fin m_Val -> Val n_Val) (s : Tm m_Val) {struct s} : Tm n_Val :=
+  match s with
+  | ret _ s0 => ret n_Val (subst_Val sigma_Val s0)
+  | let_ _ s0 s1 =>
+      let_ n_Val (subst_Tm sigma_Val s0) (subst_Tm (up_Val_Val sigma_Val) s1)
+  | ifz _ s0 s1 s2 =>
+      ifz n_Val (subst_Val sigma_Val s0) (subst_Tm sigma_Val s1)
+        (subst_Tm (up_Val_Val sigma_Val) s2)
+  | prj _ s0 s1 => prj n_Val s0 (subst_Val sigma_Val s1)
+  | case _ s0 s1 s2 =>
+      case n_Val (subst_Val sigma_Val s0)
+        (subst_Tm (up_Val_Val sigma_Val) s1)
+        (subst_Tm (up_Val_Val sigma_Val) s2)
+  | app _ s0 s1 =>
+      app n_Val (subst_Val sigma_Val s0) (subst_Val sigma_Val s1)
+  | unfold _ s0 => unfold n_Val (subst_Val sigma_Val s0)
+  | raise _ s0 => raise n_Val (subst_Val sigma_Val s0)
+  | try _ s0 s1 =>
+      try n_Val (subst_Tm sigma_Val s0) (subst_Tm (up_Val_Val sigma_Val) s1)
+  | throw _ s0 s1 =>
+      throw n_Val (subst_Val sigma_Val s0) (subst_Val sigma_Val s1)
+  | letcc _ s0 => letcc n_Val (subst_Tm (up_Val_Val sigma_Val) s0)
+  | perform _ s0 => perform n_Val (subst_Val sigma_Val s0)
+  | handle _ s0 s1 s2 s3 =>
+      handle n_Val (subst_Tm sigma_Val s0)
+        (subst_Tm (up_Val_Val sigma_Val) s1) s2
+        (subst_Tm (up_Val_Val sigma_Val) s3)
+  | continue _ s0 s1 =>
+      continue n_Val (subst_Val sigma_Val s0) (subst_Val sigma_Val s1)
+  | throw_e _ s0 s1 =>
+      throw_e n_Val (subst_Val sigma_Val s0) (subst_Tm sigma_Val s1)
+  | exit _ s0 => exit n_Val (subst_Val sigma_Val s0)
+  | discontinue _ s0 s1 =>
+      discontinue n_Val (subst_Val sigma_Val s0) (subst_Val sigma_Val s1)
+  end
+with subst_Frame {m_Val : nat} {n_Val : nat}
+(sigma_Val : fin m_Val -> Val n_Val) (s : Frame m_Val) {struct s} :
+Frame n_Val :=
+  match s with
+  | f_try _ s0 => f_try n_Val (subst_Tm (up_Val_Val sigma_Val) s0)
+  | f_let _ s0 => f_let n_Val (subst_Tm (up_Val_Val sigma_Val) s0)
+  | f_handle _ s0 s1 s2 =>
+      f_handle n_Val (subst_Tm (up_Val_Val sigma_Val) s0) s1
+        (subst_Tm (up_Val_Val sigma_Val) s2)
+  end.
+
+Lemma upId_Val_Val {m_Val : nat} (sigma : fin m_Val -> Val m_Val)
+  (Eq : forall x, sigma x = var m_Val x) :
+  forall x, up_Val_Val sigma x = var (S m_Val) x.
+Proof.
+exact (fun n =>
+       match n with
+       | Some fin_n => ap (ren_Val shift) (Eq fin_n)
+       | None => eq_refl
+       end).
+Qed.
+
+Lemma upId_list_Val_Val {p : nat} {m_Val : nat}
+  (sigma : fin m_Val -> Val m_Val) (Eq : forall x, sigma x = var m_Val x) :
+  forall x, up_list_Val_Val p sigma x = var (plus p m_Val) x.
+Proof.
+exact (fun n =>
+       scons_p_eta (var (plus p m_Val))
+         (fun n => ap (ren_Val (shift_p p)) (Eq n)) (fun n => eq_refl)).
+Qed.
+
+Fixpoint idSubst_Val {m_Val : nat} (sigma_Val : fin m_Val -> Val m_Val)
+(Eq_Val : forall x, sigma_Val x = var m_Val x) (s : Val m_Val) {struct s} :
+subst_Val sigma_Val s = s :=
+  match s with
+  | var _ s0 => Eq_Val s0
+  | unit _ => congr_unit
+  | zero _ => congr_zero
+  | succ _ s0 => congr_succ (idSubst_Val sigma_Val Eq_Val s0)
+  | prod _ s0 s1 =>
+      congr_prod (idSubst_Val sigma_Val Eq_Val s0)
+        (idSubst_Val sigma_Val Eq_Val s1)
+  | inj _ s0 s1 => congr_inj (eq_refl s0) (idSubst_Val sigma_Val Eq_Val s1)
+  | abs _ s0 =>
+      congr_abs
+        (idSubst_Tm (up_Val_Val sigma_Val) (upId_Val_Val _ Eq_Val) s0)
+  | rec _ s0 =>
+      congr_rec
+        (idSubst_Val (up_Val_Val sigma_Val) (upId_Val_Val _ Eq_Val) s0)
+  | fold _ s0 => congr_fold (idSubst_Val sigma_Val Eq_Val s0)
+  | cont _ s0 => congr_cont (list_id (idSubst_Frame sigma_Val Eq_Val) s0)
+  | eff _ s0 => congr_eff (eq_refl s0)
+  | v_nil _ => congr_v_nil
+  | v_cons _ s0 s1 =>
+      congr_v_cons (idSubst_Val sigma_Val Eq_Val s0)
+        (idSubst_Val sigma_Val Eq_Val s1)
+  end
+with idSubst_Tm {m_Val : nat} (sigma_Val : fin m_Val -> Val m_Val)
+(Eq_Val : forall x, sigma_Val x = var m_Val x) (s : Tm m_Val) {struct s} :
+subst_Tm sigma_Val s = s :=
+  match s with
+  | ret _ s0 => congr_ret (idSubst_Val sigma_Val Eq_Val s0)
+  | let_ _ s0 s1 =>
+      congr_let_ (idSubst_Tm sigma_Val Eq_Val s0)
+        (idSubst_Tm (up_Val_Val sigma_Val) (upId_Val_Val _ Eq_Val) s1)
+  | ifz _ s0 s1 s2 =>
+      congr_ifz (idSubst_Val sigma_Val Eq_Val s0)
+        (idSubst_Tm sigma_Val Eq_Val s1)
+        (idSubst_Tm (up_Val_Val sigma_Val) (upId_Val_Val _ Eq_Val) s2)
+  | prj _ s0 s1 => congr_prj (eq_refl s0) (idSubst_Val sigma_Val Eq_Val s1)
+  | case _ s0 s1 s2 =>
+      congr_case (idSubst_Val sigma_Val Eq_Val s0)
+        (idSubst_Tm (up_Val_Val sigma_Val) (upId_Val_Val _ Eq_Val) s1)
+        (idSubst_Tm (up_Val_Val sigma_Val) (upId_Val_Val _ Eq_Val) s2)
+  | app _ s0 s1 =>
+      congr_app (idSubst_Val sigma_Val Eq_Val s0)
+        (idSubst_Val sigma_Val Eq_Val s1)
+  | unfold _ s0 => congr_unfold (idSubst_Val sigma_Val Eq_Val s0)
+  | raise _ s0 => congr_raise (idSubst_Val sigma_Val Eq_Val s0)
+  | try _ s0 s1 =>
+      congr_try (idSubst_Tm sigma_Val Eq_Val s0)
+        (idSubst_Tm (up_Val_Val sigma_Val) (upId_Val_Val _ Eq_Val) s1)
+  | throw _ s0 s1 =>
+      congr_throw (idSubst_Val sigma_Val Eq_Val s0)
+        (idSubst_Val sigma_Val Eq_Val s1)
+  | letcc _ s0 =>
+      congr_letcc
+        (idSubst_Tm (up_Val_Val sigma_Val) (upId_Val_Val _ Eq_Val) s0)
+  | perform _ s0 => congr_perform (idSubst_Val sigma_Val Eq_Val s0)
+  | handle _ s0 s1 s2 s3 =>
+      congr_handle (idSubst_Tm sigma_Val Eq_Val s0)
+        (idSubst_Tm (up_Val_Val sigma_Val) (upId_Val_Val _ Eq_Val) s1)
+        (eq_refl s2)
+        (idSubst_Tm (up_Val_Val sigma_Val) (upId_Val_Val _ Eq_Val) s3)
+  | continue _ s0 s1 =>
+      congr_continue (idSubst_Val sigma_Val Eq_Val s0)
+        (idSubst_Val sigma_Val Eq_Val s1)
+  | throw_e _ s0 s1 =>
+      congr_throw_e (idSubst_Val sigma_Val Eq_Val s0)
+        (idSubst_Tm sigma_Val Eq_Val s1)
+  | exit _ s0 => congr_exit (idSubst_Val sigma_Val Eq_Val s0)
+  | discontinue _ s0 s1 =>
+      congr_discontinue (idSubst_Val sigma_Val Eq_Val s0)
+        (idSubst_Val sigma_Val Eq_Val s1)
+  end
+with idSubst_Frame {m_Val : nat} (sigma_Val : fin m_Val -> Val m_Val)
+(Eq_Val : forall x, sigma_Val x = var m_Val x) (s : Frame m_Val) {struct s} :
+subst_Frame sigma_Val s = s :=
+  match s with
+  | f_try _ s0 =>
+      congr_f_try
+        (idSubst_Tm (up_Val_Val sigma_Val) (upId_Val_Val _ Eq_Val) s0)
+  | f_let _ s0 =>
+      congr_f_let
+        (idSubst_Tm (up_Val_Val sigma_Val) (upId_Val_Val _ Eq_Val) s0)
+  | f_handle _ s0 s1 s2 =>
+      congr_f_handle
+        (idSubst_Tm (up_Val_Val sigma_Val) (upId_Val_Val _ Eq_Val) s0)
+        (eq_refl s1)
+        (idSubst_Tm (up_Val_Val sigma_Val) (upId_Val_Val _ Eq_Val) s2)
+  end.
+
+Lemma upExtRen_Val_Val {m : nat} {n : nat} (xi : fin m -> fin n)
+  (zeta : fin m -> fin n) (Eq : forall x, xi x = zeta x) :
+  forall x, upRen_Val_Val xi x = upRen_Val_Val zeta x.
+Proof.
+exact (fun n =>
+       match n with
+       | Some fin_n => ap shift (Eq fin_n)
+       | None => eq_refl
+       end).
+Qed.
+
+Lemma upExtRen_list_Val_Val {p : nat} {m : nat} {n : nat}
+  (xi : fin m -> fin n) (zeta : fin m -> fin n)
+  (Eq : forall x, xi x = zeta x) :
+  forall x, upRen_list_Val_Val p xi x = upRen_list_Val_Val p zeta x.
+Proof.
+exact (fun n =>
+       scons_p_congr (fun n => eq_refl) (fun n => ap (shift_p p) (Eq n))).
+Qed.
+
+Fixpoint extRen_Val {m_Val : nat} {n_Val : nat}
+(xi_Val : fin m_Val -> fin n_Val) (zeta_Val : fin m_Val -> fin n_Val)
+(Eq_Val : forall x, xi_Val x = zeta_Val x) (s : Val m_Val) {struct s} :
+ren_Val xi_Val s = ren_Val zeta_Val s :=
+  match s with
+  | var _ s0 => ap (var n_Val) (Eq_Val s0)
+  | unit _ => congr_unit
+  | zero _ => congr_zero
+  | succ _ s0 => congr_succ (extRen_Val xi_Val zeta_Val Eq_Val s0)
+  | prod _ s0 s1 =>
+      congr_prod (extRen_Val xi_Val zeta_Val Eq_Val s0)
+        (extRen_Val xi_Val zeta_Val Eq_Val s1)
+  | inj _ s0 s1 =>
+      congr_inj (eq_refl s0) (extRen_Val xi_Val zeta_Val Eq_Val s1)
+  | abs _ s0 =>
+      congr_abs
+        (extRen_Tm (upRen_Val_Val xi_Val) (upRen_Val_Val zeta_Val)
+           (upExtRen_Val_Val _ _ Eq_Val) s0)
+  | rec _ s0 =>
+      congr_rec
+        (extRen_Val (upRen_Val_Val xi_Val) (upRen_Val_Val zeta_Val)
+           (upExtRen_Val_Val _ _ Eq_Val) s0)
+  | fold _ s0 => congr_fold (extRen_Val xi_Val zeta_Val Eq_Val s0)
+  | cont _ s0 =>
+      congr_cont (list_ext (extRen_Frame xi_Val zeta_Val Eq_Val) s0)
+  | eff _ s0 => congr_eff (eq_refl s0)
+  | v_nil _ => congr_v_nil
+  | v_cons _ s0 s1 =>
+      congr_v_cons (extRen_Val xi_Val zeta_Val Eq_Val s0)
+        (extRen_Val xi_Val zeta_Val Eq_Val s1)
+  end
+with extRen_Tm {m_Val : nat} {n_Val : nat} (xi_Val : fin m_Val -> fin n_Val)
+(zeta_Val : fin m_Val -> fin n_Val)
+(Eq_Val : forall x, xi_Val x = zeta_Val x) (s : Tm m_Val) {struct s} :
+ren_Tm xi_Val s = ren_Tm zeta_Val s :=
+  match s with
+  | ret _ s0 => congr_ret (extRen_Val xi_Val zeta_Val Eq_Val s0)
+  | let_ _ s0 s1 =>
+      congr_let_ (extRen_Tm xi_Val zeta_Val Eq_Val s0)
+        (extRen_Tm (upRen_Val_Val xi_Val) (upRen_Val_Val zeta_Val)
+           (upExtRen_Val_Val _ _ Eq_Val) s1)
+  | ifz _ s0 s1 s2 =>
+      congr_ifz (extRen_Val xi_Val zeta_Val Eq_Val s0)
+        (extRen_Tm xi_Val zeta_Val Eq_Val s1)
+        (extRen_Tm (upRen_Val_Val xi_Val) (upRen_Val_Val zeta_Val)
+           (upExtRen_Val_Val _ _ Eq_Val) s2)
+  | prj _ s0 s1 =>
+      congr_prj (eq_refl s0) (extRen_Val xi_Val zeta_Val Eq_Val s1)
+  | case _ s0 s1 s2 =>
+      congr_case (extRen_Val xi_Val zeta_Val Eq_Val s0)
+        (extRen_Tm (upRen_Val_Val xi_Val) (upRen_Val_Val zeta_Val)
+           (upExtRen_Val_Val _ _ Eq_Val) s1)
+        (extRen_Tm (upRen_Val_Val xi_Val) (upRen_Val_Val zeta_Val)
+           (upExtRen_Val_Val _ _ Eq_Val) s2)
+  | app _ s0 s1 =>
+      congr_app (extRen_Val xi_Val zeta_Val Eq_Val s0)
+        (extRen_Val xi_Val zeta_Val Eq_Val s1)
+  | unfold _ s0 => congr_unfold (extRen_Val xi_Val zeta_Val Eq_Val s0)
+  | raise _ s0 => congr_raise (extRen_Val xi_Val zeta_Val Eq_Val s0)
+  | try _ s0 s1 =>
+      congr_try (extRen_Tm xi_Val zeta_Val Eq_Val s0)
+        (extRen_Tm (upRen_Val_Val xi_Val) (upRen_Val_Val zeta_Val)
+           (upExtRen_Val_Val _ _ Eq_Val) s1)
+  | throw _ s0 s1 =>
+      congr_throw (extRen_Val xi_Val zeta_Val Eq_Val s0)
+        (extRen_Val xi_Val zeta_Val Eq_Val s1)
+  | letcc _ s0 =>
+      congr_letcc
+        (extRen_Tm (upRen_Val_Val xi_Val) (upRen_Val_Val zeta_Val)
+           (upExtRen_Val_Val _ _ Eq_Val) s0)
+  | perform _ s0 => congr_perform (extRen_Val xi_Val zeta_Val Eq_Val s0)
+  | handle _ s0 s1 s2 s3 =>
+      congr_handle (extRen_Tm xi_Val zeta_Val Eq_Val s0)
+        (extRen_Tm (upRen_Val_Val xi_Val) (upRen_Val_Val zeta_Val)
+           (upExtRen_Val_Val _ _ Eq_Val) s1)
+        (eq_refl s2)
+        (extRen_Tm (upRen_Val_Val xi_Val) (upRen_Val_Val zeta_Val)
+           (upExtRen_Val_Val _ _ Eq_Val) s3)
+  | continue _ s0 s1 =>
+      congr_continue (extRen_Val xi_Val zeta_Val Eq_Val s0)
+        (extRen_Val xi_Val zeta_Val Eq_Val s1)
+  | throw_e _ s0 s1 =>
+      congr_throw_e (extRen_Val xi_Val zeta_Val Eq_Val s0)
+        (extRen_Tm xi_Val zeta_Val Eq_Val s1)
+  | exit _ s0 => congr_exit (extRen_Val xi_Val zeta_Val Eq_Val s0)
+  | discontinue _ s0 s1 =>
+      congr_discontinue (extRen_Val xi_Val zeta_Val Eq_Val s0)
+        (extRen_Val xi_Val zeta_Val Eq_Val s1)
+  end
+with extRen_Frame {m_Val : nat} {n_Val : nat}
+(xi_Val : fin m_Val -> fin n_Val) (zeta_Val : fin m_Val -> fin n_Val)
+(Eq_Val : forall x, xi_Val x = zeta_Val x) (s : Frame m_Val) {struct s} :
+ren_Frame xi_Val s = ren_Frame zeta_Val s :=
+  match s with
+  | f_try _ s0 =>
+      congr_f_try
+        (extRen_Tm (upRen_Val_Val xi_Val) (upRen_Val_Val zeta_Val)
+           (upExtRen_Val_Val _ _ Eq_Val) s0)
+  | f_let _ s0 =>
+      congr_f_let
+        (extRen_Tm (upRen_Val_Val xi_Val) (upRen_Val_Val zeta_Val)
+           (upExtRen_Val_Val _ _ Eq_Val) s0)
+  | f_handle _ s0 s1 s2 =>
+      congr_f_handle
+        (extRen_Tm (upRen_Val_Val xi_Val) (upRen_Val_Val zeta_Val)
+           (upExtRen_Val_Val _ _ Eq_Val) s0)
+        (eq_refl s1)
+        (extRen_Tm (upRen_Val_Val xi_Val) (upRen_Val_Val zeta_Val)
+           (upExtRen_Val_Val _ _ Eq_Val) s2)
+  end.
+
+Lemma upExt_Val_Val {m : nat} {n_Val : nat} (sigma : fin m -> Val n_Val)
+  (tau : fin m -> Val n_Val) (Eq : forall x, sigma x = tau x) :
+  forall x, up_Val_Val sigma x = up_Val_Val tau x.
+Proof.
+exact (fun n =>
+       match n with
+       | Some fin_n => ap (ren_Val shift) (Eq fin_n)
+       | None => eq_refl
+       end).
+Qed.
+
+Lemma upExt_list_Val_Val {p : nat} {m : nat} {n_Val : nat}
+  (sigma : fin m -> Val n_Val) (tau : fin m -> Val n_Val)
+  (Eq : forall x, sigma x = tau x) :
+  forall x, up_list_Val_Val p sigma x = up_list_Val_Val p tau x.
+Proof.
+exact (fun n =>
+       scons_p_congr (fun n => eq_refl)
+         (fun n => ap (ren_Val (shift_p p)) (Eq n))).
+Qed.
+
+Fixpoint ext_Val {m_Val : nat} {n_Val : nat}
+(sigma_Val : fin m_Val -> Val n_Val) (tau_Val : fin m_Val -> Val n_Val)
+(Eq_Val : forall x, sigma_Val x = tau_Val x) (s : Val m_Val) {struct s} :
+subst_Val sigma_Val s = subst_Val tau_Val s :=
+  match s with
+  | var _ s0 => Eq_Val s0
+  | unit _ => congr_unit
+  | zero _ => congr_zero
+  | succ _ s0 => congr_succ (ext_Val sigma_Val tau_Val Eq_Val s0)
+  | prod _ s0 s1 =>
+      congr_prod (ext_Val sigma_Val tau_Val Eq_Val s0)
+        (ext_Val sigma_Val tau_Val Eq_Val s1)
+  | inj _ s0 s1 =>
+      congr_inj (eq_refl s0) (ext_Val sigma_Val tau_Val Eq_Val s1)
+  | abs _ s0 =>
+      congr_abs
+        (ext_Tm (up_Val_Val sigma_Val) (up_Val_Val tau_Val)
+           (upExt_Val_Val _ _ Eq_Val) s0)
+  | rec _ s0 =>
+      congr_rec
+        (ext_Val (up_Val_Val sigma_Val) (up_Val_Val tau_Val)
+           (upExt_Val_Val _ _ Eq_Val) s0)
+  | fold _ s0 => congr_fold (ext_Val sigma_Val tau_Val Eq_Val s0)
+  | cont _ s0 =>
+      congr_cont (list_ext (ext_Frame sigma_Val tau_Val Eq_Val) s0)
+  | eff _ s0 => congr_eff (eq_refl s0)
+  | v_nil _ => congr_v_nil
+  | v_cons _ s0 s1 =>
+      congr_v_cons (ext_Val sigma_Val tau_Val Eq_Val s0)
+        (ext_Val sigma_Val tau_Val Eq_Val s1)
+  end
+with ext_Tm {m_Val : nat} {n_Val : nat} (sigma_Val : fin m_Val -> Val n_Val)
+(tau_Val : fin m_Val -> Val n_Val)
+(Eq_Val : forall x, sigma_Val x = tau_Val x) (s : Tm m_Val) {struct s} :
+subst_Tm sigma_Val s = subst_Tm tau_Val s :=
+  match s with
+  | ret _ s0 => congr_ret (ext_Val sigma_Val tau_Val Eq_Val s0)
+  | let_ _ s0 s1 =>
+      congr_let_ (ext_Tm sigma_Val tau_Val Eq_Val s0)
+        (ext_Tm (up_Val_Val sigma_Val) (up_Val_Val tau_Val)
+           (upExt_Val_Val _ _ Eq_Val) s1)
+  | ifz _ s0 s1 s2 =>
+      congr_ifz (ext_Val sigma_Val tau_Val Eq_Val s0)
+        (ext_Tm sigma_Val tau_Val Eq_Val s1)
+        (ext_Tm (up_Val_Val sigma_Val) (up_Val_Val tau_Val)
+           (upExt_Val_Val _ _ Eq_Val) s2)
+  | prj _ s0 s1 =>
+      congr_prj (eq_refl s0) (ext_Val sigma_Val tau_Val Eq_Val s1)
+  | case _ s0 s1 s2 =>
+      congr_case (ext_Val sigma_Val tau_Val Eq_Val s0)
+        (ext_Tm (up_Val_Val sigma_Val) (up_Val_Val tau_Val)
+           (upExt_Val_Val _ _ Eq_Val) s1)
+        (ext_Tm (up_Val_Val sigma_Val) (up_Val_Val tau_Val)
+           (upExt_Val_Val _ _ Eq_Val) s2)
+  | app _ s0 s1 =>
+      congr_app (ext_Val sigma_Val tau_Val Eq_Val s0)
+        (ext_Val sigma_Val tau_Val Eq_Val s1)
+  | unfold _ s0 => congr_unfold (ext_Val sigma_Val tau_Val Eq_Val s0)
+  | raise _ s0 => congr_raise (ext_Val sigma_Val tau_Val Eq_Val s0)
+  | try _ s0 s1 =>
+      congr_try (ext_Tm sigma_Val tau_Val Eq_Val s0)
+        (ext_Tm (up_Val_Val sigma_Val) (up_Val_Val tau_Val)
+           (upExt_Val_Val _ _ Eq_Val) s1)
+  | throw _ s0 s1 =>
+      congr_throw (ext_Val sigma_Val tau_Val Eq_Val s0)
+        (ext_Val sigma_Val tau_Val Eq_Val s1)
+  | letcc _ s0 =>
+      congr_letcc
+        (ext_Tm (up_Val_Val sigma_Val) (up_Val_Val tau_Val)
+           (upExt_Val_Val _ _ Eq_Val) s0)
+  | perform _ s0 => congr_perform (ext_Val sigma_Val tau_Val Eq_Val s0)
+  | handle _ s0 s1 s2 s3 =>
+      congr_handle (ext_Tm sigma_Val tau_Val Eq_Val s0)
+        (ext_Tm (up_Val_Val sigma_Val) (up_Val_Val tau_Val)
+           (upExt_Val_Val _ _ Eq_Val) s1)
+        (eq_refl s2)
+        (ext_Tm (up_Val_Val sigma_Val) (up_Val_Val tau_Val)
+           (upExt_Val_Val _ _ Eq_Val) s3)
+  | continue _ s0 s1 =>
+      congr_continue (ext_Val sigma_Val tau_Val Eq_Val s0)
+        (ext_Val sigma_Val tau_Val Eq_Val s1)
+  | throw_e _ s0 s1 =>
+      congr_throw_e (ext_Val sigma_Val tau_Val Eq_Val s0)
+        (ext_Tm sigma_Val tau_Val Eq_Val s1)
+  | exit _ s0 => congr_exit (ext_Val sigma_Val tau_Val Eq_Val s0)
+  | discontinue _ s0 s1 =>
+      congr_discontinue (ext_Val sigma_Val tau_Val Eq_Val s0)
+        (ext_Val sigma_Val tau_Val Eq_Val s1)
+  end
+with ext_Frame {m_Val : nat} {n_Val : nat}
+(sigma_Val : fin m_Val -> Val n_Val) (tau_Val : fin m_Val -> Val n_Val)
+(Eq_Val : forall x, sigma_Val x = tau_Val x) (s : Frame m_Val) {struct s} :
+subst_Frame sigma_Val s = subst_Frame tau_Val s :=
+  match s with
+  | f_try _ s0 =>
+      congr_f_try
+        (ext_Tm (up_Val_Val sigma_Val) (up_Val_Val tau_Val)
+           (upExt_Val_Val _ _ Eq_Val) s0)
+  | f_let _ s0 =>
+      congr_f_let
+        (ext_Tm (up_Val_Val sigma_Val) (up_Val_Val tau_Val)
+           (upExt_Val_Val _ _ Eq_Val) s0)
+  | f_handle _ s0 s1 s2 =>
+      congr_f_handle
+        (ext_Tm (up_Val_Val sigma_Val) (up_Val_Val tau_Val)
+           (upExt_Val_Val _ _ Eq_Val) s0)
+        (eq_refl s1)
+        (ext_Tm (up_Val_Val sigma_Val) (up_Val_Val tau_Val)
+           (upExt_Val_Val _ _ Eq_Val) s2)
+  end.
+
+Lemma up_ren_ren_Val_Val {k : nat} {l : nat} {m : nat} (xi : fin k -> fin l)
+  (zeta : fin l -> fin m) (rho : fin k -> fin m)
+  (Eq : forall x, funcomp zeta xi x = rho x) :
+  forall x,
+  funcomp (upRen_Val_Val zeta) (upRen_Val_Val xi) x = upRen_Val_Val rho x.
+Proof.
+exact (up_ren_ren xi zeta rho Eq).
+Qed.
+
+Lemma up_ren_ren_list_Val_Val {p : nat} {k : nat} {l : nat} {m : nat}
+  (xi : fin k -> fin l) (zeta : fin l -> fin m) (rho : fin k -> fin m)
+  (Eq : forall x, funcomp zeta xi x = rho x) :
+  forall x,
+  funcomp (upRen_list_Val_Val p zeta) (upRen_list_Val_Val p xi) x =
+  upRen_list_Val_Val p rho x.
+Proof.
+exact (up_ren_ren_p Eq).
+Qed.
+
+Fixpoint compRenRen_Val {k_Val : nat} {l_Val : nat} {m_Val : nat}
+(xi_Val : fin m_Val -> fin k_Val) (zeta_Val : fin k_Val -> fin l_Val)
+(rho_Val : fin m_Val -> fin l_Val)
+(Eq_Val : forall x, funcomp zeta_Val xi_Val x = rho_Val x) (s : Val m_Val)
+{struct s} : ren_Val zeta_Val (ren_Val xi_Val s) = ren_Val rho_Val s :=
+  match s with
+  | var _ s0 => ap (var l_Val) (Eq_Val s0)
+  | unit _ => congr_unit
+  | zero _ => congr_zero
+  | succ _ s0 =>
+      congr_succ (compRenRen_Val xi_Val zeta_Val rho_Val Eq_Val s0)
+  | prod _ s0 s1 =>
+      congr_prod (compRenRen_Val xi_Val zeta_Val rho_Val Eq_Val s0)
+        (compRenRen_Val xi_Val zeta_Val rho_Val Eq_Val s1)
+  | inj _ s0 s1 =>
+      congr_inj (eq_refl s0)
+        (compRenRen_Val xi_Val zeta_Val rho_Val Eq_Val s1)
+  | abs _ s0 =>
+      congr_abs
+        (compRenRen_Tm (upRen_Val_Val xi_Val) (upRen_Val_Val zeta_Val)
+           (upRen_Val_Val rho_Val) (up_ren_ren _ _ _ Eq_Val) s0)
+  | rec _ s0 =>
+      congr_rec
+        (compRenRen_Val (upRen_Val_Val xi_Val) (upRen_Val_Val zeta_Val)
+           (upRen_Val_Val rho_Val) (up_ren_ren _ _ _ Eq_Val) s0)
+  | fold _ s0 =>
+      congr_fold (compRenRen_Val xi_Val zeta_Val rho_Val Eq_Val s0)
+  | cont _ s0 =>
+      congr_cont
+        (list_comp (compRenRen_Frame xi_Val zeta_Val rho_Val Eq_Val) s0)
+  | eff _ s0 => congr_eff (eq_refl s0)
+  | v_nil _ => congr_v_nil
+  | v_cons _ s0 s1 =>
+      congr_v_cons (compRenRen_Val xi_Val zeta_Val rho_Val Eq_Val s0)
+        (compRenRen_Val xi_Val zeta_Val rho_Val Eq_Val s1)
+  end
+with compRenRen_Tm {k_Val : nat} {l_Val : nat} {m_Val : nat}
+(xi_Val : fin m_Val -> fin k_Val) (zeta_Val : fin k_Val -> fin l_Val)
+(rho_Val : fin m_Val -> fin l_Val)
+(Eq_Val : forall x, funcomp zeta_Val xi_Val x = rho_Val x) (s : Tm m_Val)
+{struct s} : ren_Tm zeta_Val (ren_Tm xi_Val s) = ren_Tm rho_Val s :=
+  match s with
+  | ret _ s0 => congr_ret (compRenRen_Val xi_Val zeta_Val rho_Val Eq_Val s0)
+  | let_ _ s0 s1 =>
+      congr_let_ (compRenRen_Tm xi_Val zeta_Val rho_Val Eq_Val s0)
+        (compRenRen_Tm (upRen_Val_Val xi_Val) (upRen_Val_Val zeta_Val)
+           (upRen_Val_Val rho_Val) (up_ren_ren _ _ _ Eq_Val) s1)
+  | ifz _ s0 s1 s2 =>
+      congr_ifz (compRenRen_Val xi_Val zeta_Val rho_Val Eq_Val s0)
+        (compRenRen_Tm xi_Val zeta_Val rho_Val Eq_Val s1)
+        (compRenRen_Tm (upRen_Val_Val xi_Val) (upRen_Val_Val zeta_Val)
+           (upRen_Val_Val rho_Val) (up_ren_ren _ _ _ Eq_Val) s2)
+  | prj _ s0 s1 =>
+      congr_prj (eq_refl s0)
+        (compRenRen_Val xi_Val zeta_Val rho_Val Eq_Val s1)
+  | case _ s0 s1 s2 =>
+      congr_case (compRenRen_Val xi_Val zeta_Val rho_Val Eq_Val s0)
+        (compRenRen_Tm (upRen_Val_Val xi_Val) (upRen_Val_Val zeta_Val)
+           (upRen_Val_Val rho_Val) (up_ren_ren _ _ _ Eq_Val) s1)
+        (compRenRen_Tm (upRen_Val_Val xi_Val) (upRen_Val_Val zeta_Val)
+           (upRen_Val_Val rho_Val) (up_ren_ren _ _ _ Eq_Val) s2)
+  | app _ s0 s1 =>
+      congr_app (compRenRen_Val xi_Val zeta_Val rho_Val Eq_Val s0)
+        (compRenRen_Val xi_Val zeta_Val rho_Val Eq_Val s1)
+  | unfold _ s0 =>
+      congr_unfold (compRenRen_Val xi_Val zeta_Val rho_Val Eq_Val s0)
+  | raise _ s0 =>
+      congr_raise (compRenRen_Val xi_Val zeta_Val rho_Val Eq_Val s0)
+  | try _ s0 s1 =>
+      congr_try (compRenRen_Tm xi_Val zeta_Val rho_Val Eq_Val s0)
+        (compRenRen_Tm (upRen_Val_Val xi_Val) (upRen_Val_Val zeta_Val)
+           (upRen_Val_Val rho_Val) (up_ren_ren _ _ _ Eq_Val) s1)
+  | throw _ s0 s1 =>
+      congr_throw (compRenRen_Val xi_Val zeta_Val rho_Val Eq_Val s0)
+        (compRenRen_Val xi_Val zeta_Val rho_Val Eq_Val s1)
+  | letcc _ s0 =>
+      congr_letcc
+        (compRenRen_Tm (upRen_Val_Val xi_Val) (upRen_Val_Val zeta_Val)
+           (upRen_Val_Val rho_Val) (up_ren_ren _ _ _ Eq_Val) s0)
+  | perform _ s0 =>
+      congr_perform (compRenRen_Val xi_Val zeta_Val rho_Val Eq_Val s0)
+  | handle _ s0 s1 s2 s3 =>
+      congr_handle (compRenRen_Tm xi_Val zeta_Val rho_Val Eq_Val s0)
+        (compRenRen_Tm (upRen_Val_Val xi_Val) (upRen_Val_Val zeta_Val)
+           (upRen_Val_Val rho_Val) (up_ren_ren _ _ _ Eq_Val) s1)
+        (eq_refl s2)
+        (compRenRen_Tm (upRen_Val_Val xi_Val) (upRen_Val_Val zeta_Val)
+           (upRen_Val_Val rho_Val) (up_ren_ren _ _ _ Eq_Val) s3)
+  | continue _ s0 s1 =>
+      congr_continue (compRenRen_Val xi_Val zeta_Val rho_Val Eq_Val s0)
+        (compRenRen_Val xi_Val zeta_Val rho_Val Eq_Val s1)
+  | throw_e _ s0 s1 =>
+      congr_throw_e (compRenRen_Val xi_Val zeta_Val rho_Val Eq_Val s0)
+        (compRenRen_Tm xi_Val zeta_Val rho_Val Eq_Val s1)
+  | exit _ s0 =>
+      congr_exit (compRenRen_Val xi_Val zeta_Val rho_Val Eq_Val s0)
+  | discontinue _ s0 s1 =>
+      congr_discontinue (compRenRen_Val xi_Val zeta_Val rho_Val Eq_Val s0)
+        (compRenRen_Val xi_Val zeta_Val rho_Val Eq_Val s1)
+  end
+with compRenRen_Frame {k_Val : nat} {l_Val : nat} {m_Val : nat}
+(xi_Val : fin m_Val -> fin k_Val) (zeta_Val : fin k_Val -> fin l_Val)
+(rho_Val : fin m_Val -> fin l_Val)
+(Eq_Val : forall x, funcomp zeta_Val xi_Val x = rho_Val x) (s : Frame m_Val)
+{struct s} : ren_Frame zeta_Val (ren_Frame xi_Val s) = ren_Frame rho_Val s :=
+  match s with
+  | f_try _ s0 =>
+      congr_f_try
+        (compRenRen_Tm (upRen_Val_Val xi_Val) (upRen_Val_Val zeta_Val)
+           (upRen_Val_Val rho_Val) (up_ren_ren _ _ _ Eq_Val) s0)
+  | f_let _ s0 =>
+      congr_f_let
+        (compRenRen_Tm (upRen_Val_Val xi_Val) (upRen_Val_Val zeta_Val)
+           (upRen_Val_Val rho_Val) (up_ren_ren _ _ _ Eq_Val) s0)
+  | f_handle _ s0 s1 s2 =>
+      congr_f_handle
+        (compRenRen_Tm (upRen_Val_Val xi_Val) (upRen_Val_Val zeta_Val)
+           (upRen_Val_Val rho_Val) (up_ren_ren _ _ _ Eq_Val) s0)
+        (eq_refl s1)
+        (compRenRen_Tm (upRen_Val_Val xi_Val) (upRen_Val_Val zeta_Val)
+           (upRen_Val_Val rho_Val) (up_ren_ren _ _ _ Eq_Val) s2)
+  end.
+
+Lemma up_ren_subst_Val_Val {k : nat} {l : nat} {m_Val : nat}
+  (xi : fin k -> fin l) (tau : fin l -> Val m_Val)
+  (theta : fin k -> Val m_Val) (Eq : forall x, funcomp tau xi x = theta x) :
+  forall x,
+  funcomp (up_Val_Val tau) (upRen_Val_Val xi) x = up_Val_Val theta x.
+Proof.
+exact (fun n =>
+       match n with
+       | Some fin_n => ap (ren_Val shift) (Eq fin_n)
+       | None => eq_refl
+       end).
+Qed.
+
+Lemma up_ren_subst_list_Val_Val {p : nat} {k : nat} {l : nat} {m_Val : nat}
+  (xi : fin k -> fin l) (tau : fin l -> Val m_Val)
+  (theta : fin k -> Val m_Val) (Eq : forall x, funcomp tau xi x = theta x) :
+  forall x,
+  funcomp (up_list_Val_Val p tau) (upRen_list_Val_Val p xi) x =
+  up_list_Val_Val p theta x.
+Proof.
+exact (fun n =>
+       eq_trans (scons_p_comp' _ _ _ n)
+         (scons_p_congr (fun z => scons_p_head' _ _ z)
+            (fun z =>
+             eq_trans (scons_p_tail' _ _ (xi z))
+               (ap (ren_Val (shift_p p)) (Eq z))))).
+Qed.
+
+Fixpoint compRenSubst_Val {k_Val : nat} {l_Val : nat} {m_Val : nat}
+(xi_Val : fin m_Val -> fin k_Val) (tau_Val : fin k_Val -> Val l_Val)
+(theta_Val : fin m_Val -> Val l_Val)
+(Eq_Val : forall x, funcomp tau_Val xi_Val x = theta_Val x) (s : Val m_Val)
+{struct s} : subst_Val tau_Val (ren_Val xi_Val s) = subst_Val theta_Val s :=
+  match s with
+  | var _ s0 => Eq_Val s0
+  | unit _ => congr_unit
+  | zero _ => congr_zero
+  | succ _ s0 =>
+      congr_succ (compRenSubst_Val xi_Val tau_Val theta_Val Eq_Val s0)
+  | prod _ s0 s1 =>
+      congr_prod (compRenSubst_Val xi_Val tau_Val theta_Val Eq_Val s0)
+        (compRenSubst_Val xi_Val tau_Val theta_Val Eq_Val s1)
+  | inj _ s0 s1 =>
+      congr_inj (eq_refl s0)
+        (compRenSubst_Val xi_Val tau_Val theta_Val Eq_Val s1)
+  | abs _ s0 =>
+      congr_abs
+        (compRenSubst_Tm (upRen_Val_Val xi_Val) (up_Val_Val tau_Val)
+           (up_Val_Val theta_Val) (up_ren_subst_Val_Val _ _ _ Eq_Val) s0)
+  | rec _ s0 =>
+      congr_rec
+        (compRenSubst_Val (upRen_Val_Val xi_Val) (up_Val_Val tau_Val)
+           (up_Val_Val theta_Val) (up_ren_subst_Val_Val _ _ _ Eq_Val) s0)
+  | fold _ s0 =>
+      congr_fold (compRenSubst_Val xi_Val tau_Val theta_Val Eq_Val s0)
+  | cont _ s0 =>
+      congr_cont
+        (list_comp (compRenSubst_Frame xi_Val tau_Val theta_Val Eq_Val) s0)
+  | eff _ s0 => congr_eff (eq_refl s0)
+  | v_nil _ => congr_v_nil
+  | v_cons _ s0 s1 =>
+      congr_v_cons (compRenSubst_Val xi_Val tau_Val theta_Val Eq_Val s0)
+        (compRenSubst_Val xi_Val tau_Val theta_Val Eq_Val s1)
+  end
+with compRenSubst_Tm {k_Val : nat} {l_Val : nat} {m_Val : nat}
+(xi_Val : fin m_Val -> fin k_Val) (tau_Val : fin k_Val -> Val l_Val)
+(theta_Val : fin m_Val -> Val l_Val)
+(Eq_Val : forall x, funcomp tau_Val xi_Val x = theta_Val x) (s : Tm m_Val)
+{struct s} : subst_Tm tau_Val (ren_Tm xi_Val s) = subst_Tm theta_Val s :=
+  match s with
+  | ret _ s0 =>
+      congr_ret (compRenSubst_Val xi_Val tau_Val theta_Val Eq_Val s0)
+  | let_ _ s0 s1 =>
+      congr_let_ (compRenSubst_Tm xi_Val tau_Val theta_Val Eq_Val s0)
+        (compRenSubst_Tm (upRen_Val_Val xi_Val) (up_Val_Val tau_Val)
+           (up_Val_Val theta_Val) (up_ren_subst_Val_Val _ _ _ Eq_Val) s1)
+  | ifz _ s0 s1 s2 =>
+      congr_ifz (compRenSubst_Val xi_Val tau_Val theta_Val Eq_Val s0)
+        (compRenSubst_Tm xi_Val tau_Val theta_Val Eq_Val s1)
+        (compRenSubst_Tm (upRen_Val_Val xi_Val) (up_Val_Val tau_Val)
+           (up_Val_Val theta_Val) (up_ren_subst_Val_Val _ _ _ Eq_Val) s2)
+  | prj _ s0 s1 =>
+      congr_prj (eq_refl s0)
+        (compRenSubst_Val xi_Val tau_Val theta_Val Eq_Val s1)
+  | case _ s0 s1 s2 =>
+      congr_case (compRenSubst_Val xi_Val tau_Val theta_Val Eq_Val s0)
+        (compRenSubst_Tm (upRen_Val_Val xi_Val) (up_Val_Val tau_Val)
+           (up_Val_Val theta_Val) (up_ren_subst_Val_Val _ _ _ Eq_Val) s1)
+        (compRenSubst_Tm (upRen_Val_Val xi_Val) (up_Val_Val tau_Val)
+           (up_Val_Val theta_Val) (up_ren_subst_Val_Val _ _ _ Eq_Val) s2)
+  | app _ s0 s1 =>
+      congr_app (compRenSubst_Val xi_Val tau_Val theta_Val Eq_Val s0)
+        (compRenSubst_Val xi_Val tau_Val theta_Val Eq_Val s1)
+  | unfold _ s0 =>
+      congr_unfold (compRenSubst_Val xi_Val tau_Val theta_Val Eq_Val s0)
+  | raise _ s0 =>
+      congr_raise (compRenSubst_Val xi_Val tau_Val theta_Val Eq_Val s0)
+  | try _ s0 s1 =>
+      congr_try (compRenSubst_Tm xi_Val tau_Val theta_Val Eq_Val s0)
+        (compRenSubst_Tm (upRen_Val_Val xi_Val) (up_Val_Val tau_Val)
+           (up_Val_Val theta_Val) (up_ren_subst_Val_Val _ _ _ Eq_Val) s1)
+  | throw _ s0 s1 =>
+      congr_throw (compRenSubst_Val xi_Val tau_Val theta_Val Eq_Val s0)
+        (compRenSubst_Val xi_Val tau_Val theta_Val Eq_Val s1)
+  | letcc _ s0 =>
+      congr_letcc
+        (compRenSubst_Tm (upRen_Val_Val xi_Val) (up_Val_Val tau_Val)
+           (up_Val_Val theta_Val) (up_ren_subst_Val_Val _ _ _ Eq_Val) s0)
+  | perform _ s0 =>
+      congr_perform (compRenSubst_Val xi_Val tau_Val theta_Val Eq_Val s0)
+  | handle _ s0 s1 s2 s3 =>
+      congr_handle (compRenSubst_Tm xi_Val tau_Val theta_Val Eq_Val s0)
+        (compRenSubst_Tm (upRen_Val_Val xi_Val) (up_Val_Val tau_Val)
+           (up_Val_Val theta_Val) (up_ren_subst_Val_Val _ _ _ Eq_Val) s1)
+        (eq_refl s2)
+        (compRenSubst_Tm (upRen_Val_Val xi_Val) (up_Val_Val tau_Val)
+           (up_Val_Val theta_Val) (up_ren_subst_Val_Val _ _ _ Eq_Val) s3)
+  | continue _ s0 s1 =>
+      congr_continue (compRenSubst_Val xi_Val tau_Val theta_Val Eq_Val s0)
+        (compRenSubst_Val xi_Val tau_Val theta_Val Eq_Val s1)
+  | throw_e _ s0 s1 =>
+      congr_throw_e (compRenSubst_Val xi_Val tau_Val theta_Val Eq_Val s0)
+        (compRenSubst_Tm xi_Val tau_Val theta_Val Eq_Val s1)
+  | exit _ s0 =>
+      congr_exit (compRenSubst_Val xi_Val tau_Val theta_Val Eq_Val s0)
+  | discontinue _ s0 s1 =>
+      congr_discontinue (compRenSubst_Val xi_Val tau_Val theta_Val Eq_Val s0)
+        (compRenSubst_Val xi_Val tau_Val theta_Val Eq_Val s1)
+  end
+with compRenSubst_Frame {k_Val : nat} {l_Val : nat} {m_Val : nat}
+(xi_Val : fin m_Val -> fin k_Val) (tau_Val : fin k_Val -> Val l_Val)
+(theta_Val : fin m_Val -> Val l_Val)
+(Eq_Val : forall x, funcomp tau_Val xi_Val x = theta_Val x) (s : Frame m_Val)
+{struct s} :
+subst_Frame tau_Val (ren_Frame xi_Val s) = subst_Frame theta_Val s :=
+  match s with
+  | f_try _ s0 =>
+      congr_f_try
+        (compRenSubst_Tm (upRen_Val_Val xi_Val) (up_Val_Val tau_Val)
+           (up_Val_Val theta_Val) (up_ren_subst_Val_Val _ _ _ Eq_Val) s0)
+  | f_let _ s0 =>
+      congr_f_let
+        (compRenSubst_Tm (upRen_Val_Val xi_Val) (up_Val_Val tau_Val)
+           (up_Val_Val theta_Val) (up_ren_subst_Val_Val _ _ _ Eq_Val) s0)
+  | f_handle _ s0 s1 s2 =>
+      congr_f_handle
+        (compRenSubst_Tm (upRen_Val_Val xi_Val) (up_Val_Val tau_Val)
+           (up_Val_Val theta_Val) (up_ren_subst_Val_Val _ _ _ Eq_Val) s0)
+        (eq_refl s1)
+        (compRenSubst_Tm (upRen_Val_Val xi_Val) (up_Val_Val tau_Val)
+           (up_Val_Val theta_Val) (up_ren_subst_Val_Val _ _ _ Eq_Val) s2)
+  end.
+
+Lemma up_subst_ren_Val_Val {k : nat} {l_Val : nat} {m_Val : nat}
+  (sigma : fin k -> Val l_Val) (zeta_Val : fin l_Val -> fin m_Val)
+  (theta : fin k -> Val m_Val)
+  (Eq : forall x, funcomp (ren_Val zeta_Val) sigma x = theta x) :
+  forall x,
+  funcomp (ren_Val (upRen_Val_Val zeta_Val)) (up_Val_Val sigma) x =
+  up_Val_Val theta x.
+Proof.
+exact (fun n =>
+       match n with
+       | Some fin_n =>
+           eq_trans
+             (compRenRen_Val shift (upRen_Val_Val zeta_Val)
+                (funcomp shift zeta_Val) (fun x => eq_refl) (sigma fin_n))
+             (eq_trans
+                (eq_sym
+                   (compRenRen_Val zeta_Val shift (funcomp shift zeta_Val)
+                      (fun x => eq_refl) (sigma fin_n)))
+                (ap (ren_Val shift) (Eq fin_n)))
+       | None => eq_refl
+       end).
+Qed.
+
+Lemma up_subst_ren_list_Val_Val {p : nat} {k : nat} {l_Val : nat}
+  {m_Val : nat} (sigma : fin k -> Val l_Val)
+  (zeta_Val : fin l_Val -> fin m_Val) (theta : fin k -> Val m_Val)
+  (Eq : forall x, funcomp (ren_Val zeta_Val) sigma x = theta x) :
+  forall x,
+  funcomp (ren_Val (upRen_list_Val_Val p zeta_Val)) (up_list_Val_Val p sigma)
+    x =
+  up_list_Val_Val p theta x.
+Proof.
+exact (fun n =>
+       eq_trans (scons_p_comp' _ _ _ n)
+         (scons_p_congr
+            (fun x => ap (var (plus p m_Val)) (scons_p_head' _ _ x))
+            (fun n =>
+             eq_trans
+               (compRenRen_Val (shift_p p) (upRen_list_Val_Val p zeta_Val)
+                  (funcomp (shift_p p) zeta_Val)
+                  (fun x => scons_p_tail' _ _ x) (sigma n))
+               (eq_trans
+                  (eq_sym
+                     (compRenRen_Val zeta_Val (shift_p p)
+                        (funcomp (shift_p p) zeta_Val) (fun x => eq_refl)
+                        (sigma n)))
+                  (ap (ren_Val (shift_p p)) (Eq n)))))).
+Qed.
+
+Fixpoint compSubstRen_Val {k_Val : nat} {l_Val : nat} {m_Val : nat}
+(sigma_Val : fin m_Val -> Val k_Val) (zeta_Val : fin k_Val -> fin l_Val)
+(theta_Val : fin m_Val -> Val l_Val)
+(Eq_Val : forall x, funcomp (ren_Val zeta_Val) sigma_Val x = theta_Val x)
+(s : Val m_Val) {struct s} :
+ren_Val zeta_Val (subst_Val sigma_Val s) = subst_Val theta_Val s :=
+  match s with
+  | var _ s0 => Eq_Val s0
+  | unit _ => congr_unit
+  | zero _ => congr_zero
+  | succ _ s0 =>
+      congr_succ (compSubstRen_Val sigma_Val zeta_Val theta_Val Eq_Val s0)
+  | prod _ s0 s1 =>
+      congr_prod (compSubstRen_Val sigma_Val zeta_Val theta_Val Eq_Val s0)
+        (compSubstRen_Val sigma_Val zeta_Val theta_Val Eq_Val s1)
+  | inj _ s0 s1 =>
+      congr_inj (eq_refl s0)
+        (compSubstRen_Val sigma_Val zeta_Val theta_Val Eq_Val s1)
+  | abs _ s0 =>
+      congr_abs
+        (compSubstRen_Tm (up_Val_Val sigma_Val) (upRen_Val_Val zeta_Val)
+           (up_Val_Val theta_Val) (up_subst_ren_Val_Val _ _ _ Eq_Val) s0)
+  | rec _ s0 =>
+      congr_rec
+        (compSubstRen_Val (up_Val_Val sigma_Val) (upRen_Val_Val zeta_Val)
+           (up_Val_Val theta_Val) (up_subst_ren_Val_Val _ _ _ Eq_Val) s0)
+  | fold _ s0 =>
+      congr_fold (compSubstRen_Val sigma_Val zeta_Val theta_Val Eq_Val s0)
+  | cont _ s0 =>
+      congr_cont
+        (list_comp (compSubstRen_Frame sigma_Val zeta_Val theta_Val Eq_Val)
+           s0)
+  | eff _ s0 => congr_eff (eq_refl s0)
+  | v_nil _ => congr_v_nil
+  | v_cons _ s0 s1 =>
+      congr_v_cons (compSubstRen_Val sigma_Val zeta_Val theta_Val Eq_Val s0)
+        (compSubstRen_Val sigma_Val zeta_Val theta_Val Eq_Val s1)
+  end
+with compSubstRen_Tm {k_Val : nat} {l_Val : nat} {m_Val : nat}
+(sigma_Val : fin m_Val -> Val k_Val) (zeta_Val : fin k_Val -> fin l_Val)
+(theta_Val : fin m_Val -> Val l_Val)
+(Eq_Val : forall x, funcomp (ren_Val zeta_Val) sigma_Val x = theta_Val x)
+(s : Tm m_Val) {struct s} :
+ren_Tm zeta_Val (subst_Tm sigma_Val s) = subst_Tm theta_Val s :=
+  match s with
+  | ret _ s0 =>
+      congr_ret (compSubstRen_Val sigma_Val zeta_Val theta_Val Eq_Val s0)
+  | let_ _ s0 s1 =>
+      congr_let_ (compSubstRen_Tm sigma_Val zeta_Val theta_Val Eq_Val s0)
+        (compSubstRen_Tm (up_Val_Val sigma_Val) (upRen_Val_Val zeta_Val)
+           (up_Val_Val theta_Val) (up_subst_ren_Val_Val _ _ _ Eq_Val) s1)
+  | ifz _ s0 s1 s2 =>
+      congr_ifz (compSubstRen_Val sigma_Val zeta_Val theta_Val Eq_Val s0)
+        (compSubstRen_Tm sigma_Val zeta_Val theta_Val Eq_Val s1)
+        (compSubstRen_Tm (up_Val_Val sigma_Val) (upRen_Val_Val zeta_Val)
+           (up_Val_Val theta_Val) (up_subst_ren_Val_Val _ _ _ Eq_Val) s2)
+  | prj _ s0 s1 =>
+      congr_prj (eq_refl s0)
+        (compSubstRen_Val sigma_Val zeta_Val theta_Val Eq_Val s1)
+  | case _ s0 s1 s2 =>
+      congr_case (compSubstRen_Val sigma_Val zeta_Val theta_Val Eq_Val s0)
+        (compSubstRen_Tm (up_Val_Val sigma_Val) (upRen_Val_Val zeta_Val)
+           (up_Val_Val theta_Val) (up_subst_ren_Val_Val _ _ _ Eq_Val) s1)
+        (compSubstRen_Tm (up_Val_Val sigma_Val) (upRen_Val_Val zeta_Val)
+           (up_Val_Val theta_Val) (up_subst_ren_Val_Val _ _ _ Eq_Val) s2)
+  | app _ s0 s1 =>
+      congr_app (compSubstRen_Val sigma_Val zeta_Val theta_Val Eq_Val s0)
+        (compSubstRen_Val sigma_Val zeta_Val theta_Val Eq_Val s1)
+  | unfold _ s0 =>
+      congr_unfold (compSubstRen_Val sigma_Val zeta_Val theta_Val Eq_Val s0)
+  | raise _ s0 =>
+      congr_raise (compSubstRen_Val sigma_Val zeta_Val theta_Val Eq_Val s0)
+  | try _ s0 s1 =>
+      congr_try (compSubstRen_Tm sigma_Val zeta_Val theta_Val Eq_Val s0)
+        (compSubstRen_Tm (up_Val_Val sigma_Val) (upRen_Val_Val zeta_Val)
+           (up_Val_Val theta_Val) (up_subst_ren_Val_Val _ _ _ Eq_Val) s1)
+  | throw _ s0 s1 =>
+      congr_throw (compSubstRen_Val sigma_Val zeta_Val theta_Val Eq_Val s0)
+        (compSubstRen_Val sigma_Val zeta_Val theta_Val Eq_Val s1)
+  | letcc _ s0 =>
+      congr_letcc
+        (compSubstRen_Tm (up_Val_Val sigma_Val) (upRen_Val_Val zeta_Val)
+           (up_Val_Val theta_Val) (up_subst_ren_Val_Val _ _ _ Eq_Val) s0)
+  | perform _ s0 =>
+      congr_perform (compSubstRen_Val sigma_Val zeta_Val theta_Val Eq_Val s0)
+  | handle _ s0 s1 s2 s3 =>
+      congr_handle (compSubstRen_Tm sigma_Val zeta_Val theta_Val Eq_Val s0)
+        (compSubstRen_Tm (up_Val_Val sigma_Val) (upRen_Val_Val zeta_Val)
+           (up_Val_Val theta_Val) (up_subst_ren_Val_Val _ _ _ Eq_Val) s1)
+        (eq_refl s2)
+        (compSubstRen_Tm (up_Val_Val sigma_Val) (upRen_Val_Val zeta_Val)
+           (up_Val_Val theta_Val) (up_subst_ren_Val_Val _ _ _ Eq_Val) s3)
+  | continue _ s0 s1 =>
+      congr_continue
+        (compSubstRen_Val sigma_Val zeta_Val theta_Val Eq_Val s0)
+        (compSubstRen_Val sigma_Val zeta_Val theta_Val Eq_Val s1)
+  | throw_e _ s0 s1 =>
+      congr_throw_e (compSubstRen_Val sigma_Val zeta_Val theta_Val Eq_Val s0)
+        (compSubstRen_Tm sigma_Val zeta_Val theta_Val Eq_Val s1)
+  | exit _ s0 =>
+      congr_exit (compSubstRen_Val sigma_Val zeta_Val theta_Val Eq_Val s0)
+  | discontinue _ s0 s1 =>
+      congr_discontinue
+        (compSubstRen_Val sigma_Val zeta_Val theta_Val Eq_Val s0)
+        (compSubstRen_Val sigma_Val zeta_Val theta_Val Eq_Val s1)
+  end
+with compSubstRen_Frame {k_Val : nat} {l_Val : nat} {m_Val : nat}
+(sigma_Val : fin m_Val -> Val k_Val) (zeta_Val : fin k_Val -> fin l_Val)
+(theta_Val : fin m_Val -> Val l_Val)
+(Eq_Val : forall x, funcomp (ren_Val zeta_Val) sigma_Val x = theta_Val x)
+(s : Frame m_Val) {struct s} :
+ren_Frame zeta_Val (subst_Frame sigma_Val s) = subst_Frame theta_Val s :=
+  match s with
+  | f_try _ s0 =>
+      congr_f_try
+        (compSubstRen_Tm (up_Val_Val sigma_Val) (upRen_Val_Val zeta_Val)
+           (up_Val_Val theta_Val) (up_subst_ren_Val_Val _ _ _ Eq_Val) s0)
+  | f_let _ s0 =>
+      congr_f_let
+        (compSubstRen_Tm (up_Val_Val sigma_Val) (upRen_Val_Val zeta_Val)
+           (up_Val_Val theta_Val) (up_subst_ren_Val_Val _ _ _ Eq_Val) s0)
+  | f_handle _ s0 s1 s2 =>
+      congr_f_handle
+        (compSubstRen_Tm (up_Val_Val sigma_Val) (upRen_Val_Val zeta_Val)
+           (up_Val_Val theta_Val) (up_subst_ren_Val_Val _ _ _ Eq_Val) s0)
+        (eq_refl s1)
+        (compSubstRen_Tm (up_Val_Val sigma_Val) (upRen_Val_Val zeta_Val)
+           (up_Val_Val theta_Val) (up_subst_ren_Val_Val _ _ _ Eq_Val) s2)
+  end.
+
+Lemma up_subst_subst_Val_Val {k : nat} {l_Val : nat} {m_Val : nat}
+  (sigma : fin k -> Val l_Val) (tau_Val : fin l_Val -> Val m_Val)
+  (theta : fin k -> Val m_Val)
+  (Eq : forall x, funcomp (subst_Val tau_Val) sigma x = theta x) :
+  forall x,
+  funcomp (subst_Val (up_Val_Val tau_Val)) (up_Val_Val sigma) x =
+  up_Val_Val theta x.
+Proof.
+exact (fun n =>
+       match n with
+       | Some fin_n =>
+           eq_trans
+             (compRenSubst_Val shift (up_Val_Val tau_Val)
+                (funcomp (up_Val_Val tau_Val) shift) (fun x => eq_refl)
+                (sigma fin_n))
+             (eq_trans
+                (eq_sym
+                   (compSubstRen_Val tau_Val shift
+                      (funcomp (ren_Val shift) tau_Val) (fun x => eq_refl)
+                      (sigma fin_n)))
+                (ap (ren_Val shift) (Eq fin_n)))
+       | None => eq_refl
+       end).
+Qed.
+
+Lemma up_subst_subst_list_Val_Val {p : nat} {k : nat} {l_Val : nat}
+  {m_Val : nat} (sigma : fin k -> Val l_Val)
+  (tau_Val : fin l_Val -> Val m_Val) (theta : fin k -> Val m_Val)
+  (Eq : forall x, funcomp (subst_Val tau_Val) sigma x = theta x) :
+  forall x,
+  funcomp (subst_Val (up_list_Val_Val p tau_Val)) (up_list_Val_Val p sigma) x =
+  up_list_Val_Val p theta x.
+Proof.
+exact (fun n =>
+       eq_trans
+         (scons_p_comp' (funcomp (var (plus p l_Val)) (zero_p p)) _ _ n)
+         (scons_p_congr
+            (fun x => scons_p_head' _ (fun z => ren_Val (shift_p p) _) x)
+            (fun n =>
+             eq_trans
+               (compRenSubst_Val (shift_p p) (up_list_Val_Val p tau_Val)
+                  (funcomp (up_list_Val_Val p tau_Val) (shift_p p))
+                  (fun x => eq_refl) (sigma n))
+               (eq_trans
+                  (eq_sym
+                     (compSubstRen_Val tau_Val (shift_p p) _
+                        (fun x => eq_sym (scons_p_tail' _ _ x)) (sigma n)))
+                  (ap (ren_Val (shift_p p)) (Eq n)))))).
+Qed.
+
+Fixpoint compSubstSubst_Val {k_Val : nat} {l_Val : nat} {m_Val : nat}
+(sigma_Val : fin m_Val -> Val k_Val) (tau_Val : fin k_Val -> Val l_Val)
+(theta_Val : fin m_Val -> Val l_Val)
+(Eq_Val : forall x, funcomp (subst_Val tau_Val) sigma_Val x = theta_Val x)
+(s : Val m_Val) {struct s} :
+subst_Val tau_Val (subst_Val sigma_Val s) = subst_Val theta_Val s :=
+  match s with
+  | var _ s0 => Eq_Val s0
+  | unit _ => congr_unit
+  | zero _ => congr_zero
+  | succ _ s0 =>
+      congr_succ (compSubstSubst_Val sigma_Val tau_Val theta_Val Eq_Val s0)
+  | prod _ s0 s1 =>
+      congr_prod (compSubstSubst_Val sigma_Val tau_Val theta_Val Eq_Val s0)
+        (compSubstSubst_Val sigma_Val tau_Val theta_Val Eq_Val s1)
+  | inj _ s0 s1 =>
+      congr_inj (eq_refl s0)
+        (compSubstSubst_Val sigma_Val tau_Val theta_Val Eq_Val s1)
+  | abs _ s0 =>
+      congr_abs
+        (compSubstSubst_Tm (up_Val_Val sigma_Val) (up_Val_Val tau_Val)
+           (up_Val_Val theta_Val) (up_subst_subst_Val_Val _ _ _ Eq_Val) s0)
+  | rec _ s0 =>
+      congr_rec
+        (compSubstSubst_Val (up_Val_Val sigma_Val) (up_Val_Val tau_Val)
+           (up_Val_Val theta_Val) (up_subst_subst_Val_Val _ _ _ Eq_Val) s0)
+  | fold _ s0 =>
+      congr_fold (compSubstSubst_Val sigma_Val tau_Val theta_Val Eq_Val s0)
+  | cont _ s0 =>
+      congr_cont
+        (list_comp (compSubstSubst_Frame sigma_Val tau_Val theta_Val Eq_Val)
+           s0)
+  | eff _ s0 => congr_eff (eq_refl s0)
+  | v_nil _ => congr_v_nil
+  | v_cons _ s0 s1 =>
+      congr_v_cons (compSubstSubst_Val sigma_Val tau_Val theta_Val Eq_Val s0)
+        (compSubstSubst_Val sigma_Val tau_Val theta_Val Eq_Val s1)
+  end
+with compSubstSubst_Tm {k_Val : nat} {l_Val : nat} {m_Val : nat}
+(sigma_Val : fin m_Val -> Val k_Val) (tau_Val : fin k_Val -> Val l_Val)
+(theta_Val : fin m_Val -> Val l_Val)
+(Eq_Val : forall x, funcomp (subst_Val tau_Val) sigma_Val x = theta_Val x)
+(s : Tm m_Val) {struct s} :
+subst_Tm tau_Val (subst_Tm sigma_Val s) = subst_Tm theta_Val s :=
+  match s with
+  | ret _ s0 =>
+      congr_ret (compSubstSubst_Val sigma_Val tau_Val theta_Val Eq_Val s0)
+  | let_ _ s0 s1 =>
+      congr_let_ (compSubstSubst_Tm sigma_Val tau_Val theta_Val Eq_Val s0)
+        (compSubstSubst_Tm (up_Val_Val sigma_Val) (up_Val_Val tau_Val)
+           (up_Val_Val theta_Val) (up_subst_subst_Val_Val _ _ _ Eq_Val) s1)
+  | ifz _ s0 s1 s2 =>
+      congr_ifz (compSubstSubst_Val sigma_Val tau_Val theta_Val Eq_Val s0)
+        (compSubstSubst_Tm sigma_Val tau_Val theta_Val Eq_Val s1)
+        (compSubstSubst_Tm (up_Val_Val sigma_Val) (up_Val_Val tau_Val)
+           (up_Val_Val theta_Val) (up_subst_subst_Val_Val _ _ _ Eq_Val) s2)
+  | prj _ s0 s1 =>
+      congr_prj (eq_refl s0)
+        (compSubstSubst_Val sigma_Val tau_Val theta_Val Eq_Val s1)
+  | case _ s0 s1 s2 =>
+      congr_case (compSubstSubst_Val sigma_Val tau_Val theta_Val Eq_Val s0)
+        (compSubstSubst_Tm (up_Val_Val sigma_Val) (up_Val_Val tau_Val)
+           (up_Val_Val theta_Val) (up_subst_subst_Val_Val _ _ _ Eq_Val) s1)
+        (compSubstSubst_Tm (up_Val_Val sigma_Val) (up_Val_Val tau_Val)
+           (up_Val_Val theta_Val) (up_subst_subst_Val_Val _ _ _ Eq_Val) s2)
+  | app _ s0 s1 =>
+      congr_app (compSubstSubst_Val sigma_Val tau_Val theta_Val Eq_Val s0)
+        (compSubstSubst_Val sigma_Val tau_Val theta_Val Eq_Val s1)
+  | unfold _ s0 =>
+      congr_unfold (compSubstSubst_Val sigma_Val tau_Val theta_Val Eq_Val s0)
+  | raise _ s0 =>
+      congr_raise (compSubstSubst_Val sigma_Val tau_Val theta_Val Eq_Val s0)
+  | try _ s0 s1 =>
+      congr_try (compSubstSubst_Tm sigma_Val tau_Val theta_Val Eq_Val s0)
+        (compSubstSubst_Tm (up_Val_Val sigma_Val) (up_Val_Val tau_Val)
+           (up_Val_Val theta_Val) (up_subst_subst_Val_Val _ _ _ Eq_Val) s1)
+  | throw _ s0 s1 =>
+      congr_throw (compSubstSubst_Val sigma_Val tau_Val theta_Val Eq_Val s0)
+        (compSubstSubst_Val sigma_Val tau_Val theta_Val Eq_Val s1)
+  | letcc _ s0 =>
+      congr_letcc
+        (compSubstSubst_Tm (up_Val_Val sigma_Val) (up_Val_Val tau_Val)
+           (up_Val_Val theta_Val) (up_subst_subst_Val_Val _ _ _ Eq_Val) s0)
+  | perform _ s0 =>
+      congr_perform
+        (compSubstSubst_Val sigma_Val tau_Val theta_Val Eq_Val s0)
+  | handle _ s0 s1 s2 s3 =>
+      congr_handle (compSubstSubst_Tm sigma_Val tau_Val theta_Val Eq_Val s0)
+        (compSubstSubst_Tm (up_Val_Val sigma_Val) (up_Val_Val tau_Val)
+           (up_Val_Val theta_Val) (up_subst_subst_Val_Val _ _ _ Eq_Val) s1)
+        (eq_refl s2)
+        (compSubstSubst_Tm (up_Val_Val sigma_Val) (up_Val_Val tau_Val)
+           (up_Val_Val theta_Val) (up_subst_subst_Val_Val _ _ _ Eq_Val) s3)
+  | continue _ s0 s1 =>
+      congr_continue
+        (compSubstSubst_Val sigma_Val tau_Val theta_Val Eq_Val s0)
+        (compSubstSubst_Val sigma_Val tau_Val theta_Val Eq_Val s1)
+  | throw_e _ s0 s1 =>
+      congr_throw_e
+        (compSubstSubst_Val sigma_Val tau_Val theta_Val Eq_Val s0)
+        (compSubstSubst_Tm sigma_Val tau_Val theta_Val Eq_Val s1)
+  | exit _ s0 =>
+      congr_exit (compSubstSubst_Val sigma_Val tau_Val theta_Val Eq_Val s0)
+  | discontinue _ s0 s1 =>
+      congr_discontinue
+        (compSubstSubst_Val sigma_Val tau_Val theta_Val Eq_Val s0)
+        (compSubstSubst_Val sigma_Val tau_Val theta_Val Eq_Val s1)
+  end
+with compSubstSubst_Frame {k_Val : nat} {l_Val : nat} {m_Val : nat}
+(sigma_Val : fin m_Val -> Val k_Val) (tau_Val : fin k_Val -> Val l_Val)
+(theta_Val : fin m_Val -> Val l_Val)
+(Eq_Val : forall x, funcomp (subst_Val tau_Val) sigma_Val x = theta_Val x)
+(s : Frame m_Val) {struct s} :
+subst_Frame tau_Val (subst_Frame sigma_Val s) = subst_Frame theta_Val s :=
+  match s with
+  | f_try _ s0 =>
+      congr_f_try
+        (compSubstSubst_Tm (up_Val_Val sigma_Val) (up_Val_Val tau_Val)
+           (up_Val_Val theta_Val) (up_subst_subst_Val_Val _ _ _ Eq_Val) s0)
+  | f_let _ s0 =>
+      congr_f_let
+        (compSubstSubst_Tm (up_Val_Val sigma_Val) (up_Val_Val tau_Val)
+           (up_Val_Val theta_Val) (up_subst_subst_Val_Val _ _ _ Eq_Val) s0)
+  | f_handle _ s0 s1 s2 =>
+      congr_f_handle
+        (compSubstSubst_Tm (up_Val_Val sigma_Val) (up_Val_Val tau_Val)
+           (up_Val_Val theta_Val) (up_subst_subst_Val_Val _ _ _ Eq_Val) s0)
+        (eq_refl s1)
+        (compSubstSubst_Tm (up_Val_Val sigma_Val) (up_Val_Val tau_Val)
+           (up_Val_Val theta_Val) (up_subst_subst_Val_Val _ _ _ Eq_Val) s2)
+  end.
+
+Lemma renRen_Val {k_Val : nat} {l_Val : nat} {m_Val : nat}
+  (xi_Val : fin m_Val -> fin k_Val) (zeta_Val : fin k_Val -> fin l_Val)
+  (s : Val m_Val) :
+  ren_Val zeta_Val (ren_Val xi_Val s) = ren_Val (funcomp zeta_Val xi_Val) s.
+Proof.
+exact (compRenRen_Val xi_Val zeta_Val _ (fun n => eq_refl) s).
+Qed.
+
+Lemma renRen'_Val_pointwise {k_Val : nat} {l_Val : nat} {m_Val : nat}
+  (xi_Val : fin m_Val -> fin k_Val) (zeta_Val : fin k_Val -> fin l_Val) :
+  pointwise_relation _ eq (funcomp (ren_Val zeta_Val) (ren_Val xi_Val))
+    (ren_Val (funcomp zeta_Val xi_Val)).
+Proof.
+exact (fun s => compRenRen_Val xi_Val zeta_Val _ (fun n => eq_refl) s).
+Qed.
+
+Lemma renRen_Tm {k_Val : nat} {l_Val : nat} {m_Val : nat}
+  (xi_Val : fin m_Val -> fin k_Val) (zeta_Val : fin k_Val -> fin l_Val)
+  (s : Tm m_Val) :
+  ren_Tm zeta_Val (ren_Tm xi_Val s) = ren_Tm (funcomp zeta_Val xi_Val) s.
+Proof.
+exact (compRenRen_Tm xi_Val zeta_Val _ (fun n => eq_refl) s).
+Qed.
+
+Lemma renRen'_Tm_pointwise {k_Val : nat} {l_Val : nat} {m_Val : nat}
+  (xi_Val : fin m_Val -> fin k_Val) (zeta_Val : fin k_Val -> fin l_Val) :
+  pointwise_relation _ eq (funcomp (ren_Tm zeta_Val) (ren_Tm xi_Val))
+    (ren_Tm (funcomp zeta_Val xi_Val)).
+Proof.
+exact (fun s => compRenRen_Tm xi_Val zeta_Val _ (fun n => eq_refl) s).
+Qed.
+
+Lemma renRen_Frame {k_Val : nat} {l_Val : nat} {m_Val : nat}
+  (xi_Val : fin m_Val -> fin k_Val) (zeta_Val : fin k_Val -> fin l_Val)
+  (s : Frame m_Val) :
+  ren_Frame zeta_Val (ren_Frame xi_Val s) =
+  ren_Frame (funcomp zeta_Val xi_Val) s.
+Proof.
+exact (compRenRen_Frame xi_Val zeta_Val _ (fun n => eq_refl) s).
+Qed.
+
+Lemma renRen'_Frame_pointwise {k_Val : nat} {l_Val : nat} {m_Val : nat}
+  (xi_Val : fin m_Val -> fin k_Val) (zeta_Val : fin k_Val -> fin l_Val) :
+  pointwise_relation _ eq (funcomp (ren_Frame zeta_Val) (ren_Frame xi_Val))
+    (ren_Frame (funcomp zeta_Val xi_Val)).
+Proof.
+exact (fun s => compRenRen_Frame xi_Val zeta_Val _ (fun n => eq_refl) s).
+Qed.
+
+Lemma renSubst_Val {k_Val : nat} {l_Val : nat} {m_Val : nat}
+  (xi_Val : fin m_Val -> fin k_Val) (tau_Val : fin k_Val -> Val l_Val)
+  (s : Val m_Val) :
+  subst_Val tau_Val (ren_Val xi_Val s) = subst_Val (funcomp tau_Val xi_Val) s.
+Proof.
+exact (compRenSubst_Val xi_Val tau_Val _ (fun n => eq_refl) s).
+Qed.
+
+Lemma renSubst_Val_pointwise {k_Val : nat} {l_Val : nat} {m_Val : nat}
+  (xi_Val : fin m_Val -> fin k_Val) (tau_Val : fin k_Val -> Val l_Val) :
+  pointwise_relation _ eq (funcomp (subst_Val tau_Val) (ren_Val xi_Val))
+    (subst_Val (funcomp tau_Val xi_Val)).
+Proof.
+exact (fun s => compRenSubst_Val xi_Val tau_Val _ (fun n => eq_refl) s).
+Qed.
+
+Lemma renSubst_Tm {k_Val : nat} {l_Val : nat} {m_Val : nat}
+  (xi_Val : fin m_Val -> fin k_Val) (tau_Val : fin k_Val -> Val l_Val)
+  (s : Tm m_Val) :
+  subst_Tm tau_Val (ren_Tm xi_Val s) = subst_Tm (funcomp tau_Val xi_Val) s.
+Proof.
+exact (compRenSubst_Tm xi_Val tau_Val _ (fun n => eq_refl) s).
+Qed.
+
+Lemma renSubst_Tm_pointwise {k_Val : nat} {l_Val : nat} {m_Val : nat}
+  (xi_Val : fin m_Val -> fin k_Val) (tau_Val : fin k_Val -> Val l_Val) :
+  pointwise_relation _ eq (funcomp (subst_Tm tau_Val) (ren_Tm xi_Val))
+    (subst_Tm (funcomp tau_Val xi_Val)).
+Proof.
+exact (fun s => compRenSubst_Tm xi_Val tau_Val _ (fun n => eq_refl) s).
+Qed.
+
+Lemma renSubst_Frame {k_Val : nat} {l_Val : nat} {m_Val : nat}
+  (xi_Val : fin m_Val -> fin k_Val) (tau_Val : fin k_Val -> Val l_Val)
+  (s : Frame m_Val) :
+  subst_Frame tau_Val (ren_Frame xi_Val s) =
+  subst_Frame (funcomp tau_Val xi_Val) s.
+Proof.
+exact (compRenSubst_Frame xi_Val tau_Val _ (fun n => eq_refl) s).
+Qed.
+
+Lemma renSubst_Frame_pointwise {k_Val : nat} {l_Val : nat} {m_Val : nat}
+  (xi_Val : fin m_Val -> fin k_Val) (tau_Val : fin k_Val -> Val l_Val) :
+  pointwise_relation _ eq (funcomp (subst_Frame tau_Val) (ren_Frame xi_Val))
+    (subst_Frame (funcomp tau_Val xi_Val)).
+Proof.
+exact (fun s => compRenSubst_Frame xi_Val tau_Val _ (fun n => eq_refl) s).
+Qed.
+
+Lemma substRen_Val {k_Val : nat} {l_Val : nat} {m_Val : nat}
+  (sigma_Val : fin m_Val -> Val k_Val) (zeta_Val : fin k_Val -> fin l_Val)
+  (s : Val m_Val) :
+  ren_Val zeta_Val (subst_Val sigma_Val s) =
+  subst_Val (funcomp (ren_Val zeta_Val) sigma_Val) s.
+Proof.
+exact (compSubstRen_Val sigma_Val zeta_Val _ (fun n => eq_refl) s).
+Qed.
+
+Lemma substRen_Val_pointwise {k_Val : nat} {l_Val : nat} {m_Val : nat}
+  (sigma_Val : fin m_Val -> Val k_Val) (zeta_Val : fin k_Val -> fin l_Val) :
+  pointwise_relation _ eq (funcomp (ren_Val zeta_Val) (subst_Val sigma_Val))
+    (subst_Val (funcomp (ren_Val zeta_Val) sigma_Val)).
+Proof.
+exact (fun s => compSubstRen_Val sigma_Val zeta_Val _ (fun n => eq_refl) s).
+Qed.
+
+Lemma substRen_Tm {k_Val : nat} {l_Val : nat} {m_Val : nat}
+  (sigma_Val : fin m_Val -> Val k_Val) (zeta_Val : fin k_Val -> fin l_Val)
+  (s : Tm m_Val) :
+  ren_Tm zeta_Val (subst_Tm sigma_Val s) =
+  subst_Tm (funcomp (ren_Val zeta_Val) sigma_Val) s.
+Proof.
+exact (compSubstRen_Tm sigma_Val zeta_Val _ (fun n => eq_refl) s).
+Qed.
+
+Lemma substRen_Tm_pointwise {k_Val : nat} {l_Val : nat} {m_Val : nat}
+  (sigma_Val : fin m_Val -> Val k_Val) (zeta_Val : fin k_Val -> fin l_Val) :
+  pointwise_relation _ eq (funcomp (ren_Tm zeta_Val) (subst_Tm sigma_Val))
+    (subst_Tm (funcomp (ren_Val zeta_Val) sigma_Val)).
+Proof.
+exact (fun s => compSubstRen_Tm sigma_Val zeta_Val _ (fun n => eq_refl) s).
+Qed.
+
+Lemma substRen_Frame {k_Val : nat} {l_Val : nat} {m_Val : nat}
+  (sigma_Val : fin m_Val -> Val k_Val) (zeta_Val : fin k_Val -> fin l_Val)
+  (s : Frame m_Val) :
+  ren_Frame zeta_Val (subst_Frame sigma_Val s) =
+  subst_Frame (funcomp (ren_Val zeta_Val) sigma_Val) s.
+Proof.
+exact (compSubstRen_Frame sigma_Val zeta_Val _ (fun n => eq_refl) s).
+Qed.
+
+Lemma substRen_Frame_pointwise {k_Val : nat} {l_Val : nat} {m_Val : nat}
+  (sigma_Val : fin m_Val -> Val k_Val) (zeta_Val : fin k_Val -> fin l_Val) :
+  pointwise_relation _ eq
+    (funcomp (ren_Frame zeta_Val) (subst_Frame sigma_Val))
+    (subst_Frame (funcomp (ren_Val zeta_Val) sigma_Val)).
+Proof.
+exact (fun s => compSubstRen_Frame sigma_Val zeta_Val _ (fun n => eq_refl) s).
+Qed.
+
+Lemma substSubst_Val {k_Val : nat} {l_Val : nat} {m_Val : nat}
+  (sigma_Val : fin m_Val -> Val k_Val) (tau_Val : fin k_Val -> Val l_Val)
+  (s : Val m_Val) :
+  subst_Val tau_Val (subst_Val sigma_Val s) =
+  subst_Val (funcomp (subst_Val tau_Val) sigma_Val) s.
+Proof.
+exact (compSubstSubst_Val sigma_Val tau_Val _ (fun n => eq_refl) s).
+Qed.
+
+Lemma substSubst_Val_pointwise {k_Val : nat} {l_Val : nat} {m_Val : nat}
+  (sigma_Val : fin m_Val -> Val k_Val) (tau_Val : fin k_Val -> Val l_Val) :
+  pointwise_relation _ eq (funcomp (subst_Val tau_Val) (subst_Val sigma_Val))
+    (subst_Val (funcomp (subst_Val tau_Val) sigma_Val)).
+Proof.
+exact (fun s => compSubstSubst_Val sigma_Val tau_Val _ (fun n => eq_refl) s).
+Qed.
+
+Lemma substSubst_Tm {k_Val : nat} {l_Val : nat} {m_Val : nat}
+  (sigma_Val : fin m_Val -> Val k_Val) (tau_Val : fin k_Val -> Val l_Val)
+  (s : Tm m_Val) :
+  subst_Tm tau_Val (subst_Tm sigma_Val s) =
+  subst_Tm (funcomp (subst_Val tau_Val) sigma_Val) s.
+Proof.
+exact (compSubstSubst_Tm sigma_Val tau_Val _ (fun n => eq_refl) s).
+Qed.
+
+Lemma substSubst_Tm_pointwise {k_Val : nat} {l_Val : nat} {m_Val : nat}
+  (sigma_Val : fin m_Val -> Val k_Val) (tau_Val : fin k_Val -> Val l_Val) :
+  pointwise_relation _ eq (funcomp (subst_Tm tau_Val) (subst_Tm sigma_Val))
+    (subst_Tm (funcomp (subst_Val tau_Val) sigma_Val)).
+Proof.
+exact (fun s => compSubstSubst_Tm sigma_Val tau_Val _ (fun n => eq_refl) s).
+Qed.
+
+Lemma substSubst_Frame {k_Val : nat} {l_Val : nat} {m_Val : nat}
+  (sigma_Val : fin m_Val -> Val k_Val) (tau_Val : fin k_Val -> Val l_Val)
+  (s : Frame m_Val) :
+  subst_Frame tau_Val (subst_Frame sigma_Val s) =
+  subst_Frame (funcomp (subst_Val tau_Val) sigma_Val) s.
+Proof.
+exact (compSubstSubst_Frame sigma_Val tau_Val _ (fun n => eq_refl) s).
+Qed.
+
+Lemma substSubst_Frame_pointwise {k_Val : nat} {l_Val : nat} {m_Val : nat}
+  (sigma_Val : fin m_Val -> Val k_Val) (tau_Val : fin k_Val -> Val l_Val) :
+  pointwise_relation _ eq
+    (funcomp (subst_Frame tau_Val) (subst_Frame sigma_Val))
+    (subst_Frame (funcomp (subst_Val tau_Val) sigma_Val)).
+Proof.
+exact (fun s => compSubstSubst_Frame sigma_Val tau_Val _ (fun n => eq_refl) s).
+Qed.
+
+Lemma rinstInst_up_Val_Val {m : nat} {n_Val : nat} (xi : fin m -> fin n_Val)
+  (sigma : fin m -> Val n_Val)
+  (Eq : forall x, funcomp (var n_Val) xi x = sigma x) :
+  forall x, funcomp (var (S n_Val)) (upRen_Val_Val xi) x = up_Val_Val sigma x.
+Proof.
+exact (fun n =>
+       match n with
+       | Some fin_n => ap (ren_Val shift) (Eq fin_n)
+       | None => eq_refl
+       end).
+Qed.
+
+Lemma rinstInst_up_list_Val_Val {p : nat} {m : nat} {n_Val : nat}
+  (xi : fin m -> fin n_Val) (sigma : fin m -> Val n_Val)
+  (Eq : forall x, funcomp (var n_Val) xi x = sigma x) :
+  forall x,
+  funcomp (var (plus p n_Val)) (upRen_list_Val_Val p xi) x =
+  up_list_Val_Val p sigma x.
+Proof.
+exact (fun n =>
+       eq_trans (scons_p_comp' _ _ (var (plus p n_Val)) n)
+         (scons_p_congr (fun z => eq_refl)
+            (fun n => ap (ren_Val (shift_p p)) (Eq n)))).
+Qed.
+
+Fixpoint rinst_inst_Val {m_Val : nat} {n_Val : nat}
+(xi_Val : fin m_Val -> fin n_Val) (sigma_Val : fin m_Val -> Val n_Val)
+(Eq_Val : forall x, funcomp (var n_Val) xi_Val x = sigma_Val x)
+(s : Val m_Val) {struct s} : ren_Val xi_Val s = subst_Val sigma_Val s :=
+  match s with
+  | var _ s0 => Eq_Val s0
+  | unit _ => congr_unit
+  | zero _ => congr_zero
+  | succ _ s0 => congr_succ (rinst_inst_Val xi_Val sigma_Val Eq_Val s0)
+  | prod _ s0 s1 =>
+      congr_prod (rinst_inst_Val xi_Val sigma_Val Eq_Val s0)
+        (rinst_inst_Val xi_Val sigma_Val Eq_Val s1)
+  | inj _ s0 s1 =>
+      congr_inj (eq_refl s0) (rinst_inst_Val xi_Val sigma_Val Eq_Val s1)
+  | abs _ s0 =>
+      congr_abs
+        (rinst_inst_Tm (upRen_Val_Val xi_Val) (up_Val_Val sigma_Val)
+           (rinstInst_up_Val_Val _ _ Eq_Val) s0)
+  | rec _ s0 =>
+      congr_rec
+        (rinst_inst_Val (upRen_Val_Val xi_Val) (up_Val_Val sigma_Val)
+           (rinstInst_up_Val_Val _ _ Eq_Val) s0)
+  | fold _ s0 => congr_fold (rinst_inst_Val xi_Val sigma_Val Eq_Val s0)
+  | cont _ s0 =>
+      congr_cont (list_ext (rinst_inst_Frame xi_Val sigma_Val Eq_Val) s0)
+  | eff _ s0 => congr_eff (eq_refl s0)
+  | v_nil _ => congr_v_nil
+  | v_cons _ s0 s1 =>
+      congr_v_cons (rinst_inst_Val xi_Val sigma_Val Eq_Val s0)
+        (rinst_inst_Val xi_Val sigma_Val Eq_Val s1)
+  end
+with rinst_inst_Tm {m_Val : nat} {n_Val : nat}
+(xi_Val : fin m_Val -> fin n_Val) (sigma_Val : fin m_Val -> Val n_Val)
+(Eq_Val : forall x, funcomp (var n_Val) xi_Val x = sigma_Val x)
+(s : Tm m_Val) {struct s} : ren_Tm xi_Val s = subst_Tm sigma_Val s :=
+  match s with
+  | ret _ s0 => congr_ret (rinst_inst_Val xi_Val sigma_Val Eq_Val s0)
+  | let_ _ s0 s1 =>
+      congr_let_ (rinst_inst_Tm xi_Val sigma_Val Eq_Val s0)
+        (rinst_inst_Tm (upRen_Val_Val xi_Val) (up_Val_Val sigma_Val)
+           (rinstInst_up_Val_Val _ _ Eq_Val) s1)
+  | ifz _ s0 s1 s2 =>
+      congr_ifz (rinst_inst_Val xi_Val sigma_Val Eq_Val s0)
+        (rinst_inst_Tm xi_Val sigma_Val Eq_Val s1)
+        (rinst_inst_Tm (upRen_Val_Val xi_Val) (up_Val_Val sigma_Val)
+           (rinstInst_up_Val_Val _ _ Eq_Val) s2)
+  | prj _ s0 s1 =>
+      congr_prj (eq_refl s0) (rinst_inst_Val xi_Val sigma_Val Eq_Val s1)
+  | case _ s0 s1 s2 =>
+      congr_case (rinst_inst_Val xi_Val sigma_Val Eq_Val s0)
+        (rinst_inst_Tm (upRen_Val_Val xi_Val) (up_Val_Val sigma_Val)
+           (rinstInst_up_Val_Val _ _ Eq_Val) s1)
+        (rinst_inst_Tm (upRen_Val_Val xi_Val) (up_Val_Val sigma_Val)
+           (rinstInst_up_Val_Val _ _ Eq_Val) s2)
+  | app _ s0 s1 =>
+      congr_app (rinst_inst_Val xi_Val sigma_Val Eq_Val s0)
+        (rinst_inst_Val xi_Val sigma_Val Eq_Val s1)
+  | unfold _ s0 => congr_unfold (rinst_inst_Val xi_Val sigma_Val Eq_Val s0)
+  | raise _ s0 => congr_raise (rinst_inst_Val xi_Val sigma_Val Eq_Val s0)
+  | try _ s0 s1 =>
+      congr_try (rinst_inst_Tm xi_Val sigma_Val Eq_Val s0)
+        (rinst_inst_Tm (upRen_Val_Val xi_Val) (up_Val_Val sigma_Val)
+           (rinstInst_up_Val_Val _ _ Eq_Val) s1)
+  | throw _ s0 s1 =>
+      congr_throw (rinst_inst_Val xi_Val sigma_Val Eq_Val s0)
+        (rinst_inst_Val xi_Val sigma_Val Eq_Val s1)
+  | letcc _ s0 =>
+      congr_letcc
+        (rinst_inst_Tm (upRen_Val_Val xi_Val) (up_Val_Val sigma_Val)
+           (rinstInst_up_Val_Val _ _ Eq_Val) s0)
+  | perform _ s0 => congr_perform (rinst_inst_Val xi_Val sigma_Val Eq_Val s0)
+  | handle _ s0 s1 s2 s3 =>
+      congr_handle (rinst_inst_Tm xi_Val sigma_Val Eq_Val s0)
+        (rinst_inst_Tm (upRen_Val_Val xi_Val) (up_Val_Val sigma_Val)
+           (rinstInst_up_Val_Val _ _ Eq_Val) s1)
+        (eq_refl s2)
+        (rinst_inst_Tm (upRen_Val_Val xi_Val) (up_Val_Val sigma_Val)
+           (rinstInst_up_Val_Val _ _ Eq_Val) s3)
+  | continue _ s0 s1 =>
+      congr_continue (rinst_inst_Val xi_Val sigma_Val Eq_Val s0)
+        (rinst_inst_Val xi_Val sigma_Val Eq_Val s1)
+  | throw_e _ s0 s1 =>
+      congr_throw_e (rinst_inst_Val xi_Val sigma_Val Eq_Val s0)
+        (rinst_inst_Tm xi_Val sigma_Val Eq_Val s1)
+  | exit _ s0 => congr_exit (rinst_inst_Val xi_Val sigma_Val Eq_Val s0)
+  | discontinue _ s0 s1 =>
+      congr_discontinue (rinst_inst_Val xi_Val sigma_Val Eq_Val s0)
+        (rinst_inst_Val xi_Val sigma_Val Eq_Val s1)
+  end
+with rinst_inst_Frame {m_Val : nat} {n_Val : nat}
+(xi_Val : fin m_Val -> fin n_Val) (sigma_Val : fin m_Val -> Val n_Val)
+(Eq_Val : forall x, funcomp (var n_Val) xi_Val x = sigma_Val x)
+(s : Frame m_Val) {struct s} : ren_Frame xi_Val s = subst_Frame sigma_Val s
+:=
+  match s with
+  | f_try _ s0 =>
+      congr_f_try
+        (rinst_inst_Tm (upRen_Val_Val xi_Val) (up_Val_Val sigma_Val)
+           (rinstInst_up_Val_Val _ _ Eq_Val) s0)
+  | f_let _ s0 =>
+      congr_f_let
+        (rinst_inst_Tm (upRen_Val_Val xi_Val) (up_Val_Val sigma_Val)
+           (rinstInst_up_Val_Val _ _ Eq_Val) s0)
+  | f_handle _ s0 s1 s2 =>
+      congr_f_handle
+        (rinst_inst_Tm (upRen_Val_Val xi_Val) (up_Val_Val sigma_Val)
+           (rinstInst_up_Val_Val _ _ Eq_Val) s0)
+        (eq_refl s1)
+        (rinst_inst_Tm (upRen_Val_Val xi_Val) (up_Val_Val sigma_Val)
+           (rinstInst_up_Val_Val _ _ Eq_Val) s2)
+  end.
+
+Lemma rinstInst'_Val {m_Val : nat} {n_Val : nat}
+  (xi_Val : fin m_Val -> fin n_Val) (s : Val m_Val) :
+  ren_Val xi_Val s = subst_Val (funcomp (var n_Val) xi_Val) s.
+Proof.
+exact (rinst_inst_Val xi_Val _ (fun n => eq_refl) s).
+Qed.
+
+Lemma rinstInst'_Val_pointwise {m_Val : nat} {n_Val : nat}
+  (xi_Val : fin m_Val -> fin n_Val) :
+  pointwise_relation _ eq (ren_Val xi_Val)
+    (subst_Val (funcomp (var n_Val) xi_Val)).
+Proof.
+exact (fun s => rinst_inst_Val xi_Val _ (fun n => eq_refl) s).
+Qed.
+
+Lemma rinstInst'_Tm {m_Val : nat} {n_Val : nat}
+  (xi_Val : fin m_Val -> fin n_Val) (s : Tm m_Val) :
+  ren_Tm xi_Val s = subst_Tm (funcomp (var n_Val) xi_Val) s.
+Proof.
+exact (rinst_inst_Tm xi_Val _ (fun n => eq_refl) s).
+Qed.
+
+Lemma rinstInst'_Tm_pointwise {m_Val : nat} {n_Val : nat}
+  (xi_Val : fin m_Val -> fin n_Val) :
+  pointwise_relation _ eq (ren_Tm xi_Val)
+    (subst_Tm (funcomp (var n_Val) xi_Val)).
+Proof.
+exact (fun s => rinst_inst_Tm xi_Val _ (fun n => eq_refl) s).
+Qed.
+
+Lemma rinstInst'_Frame {m_Val : nat} {n_Val : nat}
+  (xi_Val : fin m_Val -> fin n_Val) (s : Frame m_Val) :
+  ren_Frame xi_Val s = subst_Frame (funcomp (var n_Val) xi_Val) s.
+Proof.
+exact (rinst_inst_Frame xi_Val _ (fun n => eq_refl) s).
+Qed.
+
+Lemma rinstInst'_Frame_pointwise {m_Val : nat} {n_Val : nat}
+  (xi_Val : fin m_Val -> fin n_Val) :
+  pointwise_relation _ eq (ren_Frame xi_Val)
+    (subst_Frame (funcomp (var n_Val) xi_Val)).
+Proof.
+exact (fun s => rinst_inst_Frame xi_Val _ (fun n => eq_refl) s).
+Qed.
+
+Lemma instId'_Val {m_Val : nat} (s : Val m_Val) : subst_Val (var m_Val) s = s.
+Proof.
+exact (idSubst_Val (var m_Val) (fun n => eq_refl) s).
+Qed.
+
+Lemma instId'_Val_pointwise {m_Val : nat} :
+  pointwise_relation _ eq (subst_Val (var m_Val)) id.
+Proof.
+exact (fun s => idSubst_Val (var m_Val) (fun n => eq_refl) s).
+Qed.
+
+Lemma instId'_Tm {m_Val : nat} (s : Tm m_Val) : subst_Tm (var m_Val) s = s.
+Proof.
+exact (idSubst_Tm (var m_Val) (fun n => eq_refl) s).
+Qed.
+
+Lemma instId'_Tm_pointwise {m_Val : nat} :
+  pointwise_relation _ eq (subst_Tm (var m_Val)) id.
+Proof.
+exact (fun s => idSubst_Tm (var m_Val) (fun n => eq_refl) s).
+Qed.
+
+Lemma instId'_Frame {m_Val : nat} (s : Frame m_Val) :
+  subst_Frame (var m_Val) s = s.
+Proof.
+exact (idSubst_Frame (var m_Val) (fun n => eq_refl) s).
+Qed.
+
+Lemma instId'_Frame_pointwise {m_Val : nat} :
+  pointwise_relation _ eq (subst_Frame (var m_Val)) id.
+Proof.
+exact (fun s => idSubst_Frame (var m_Val) (fun n => eq_refl) s).
+Qed.
+
+Lemma rinstId'_Val {m_Val : nat} (s : Val m_Val) : ren_Val id s = s.
+Proof.
+exact (eq_ind_r (fun t => t = s) (instId'_Val s) (rinstInst'_Val id s)).
+Qed.
+
+Lemma rinstId'_Val_pointwise {m_Val : nat} :
+  pointwise_relation _ eq (@ren_Val m_Val m_Val id) id.
+Proof.
+exact (fun s =>
+       eq_ind_r (fun t => t = s) (instId'_Val s) (rinstInst'_Val id s)).
+Qed.
+
+Lemma rinstId'_Tm {m_Val : nat} (s : Tm m_Val) : ren_Tm id s = s.
+Proof.
+exact (eq_ind_r (fun t => t = s) (instId'_Tm s) (rinstInst'_Tm id s)).
+Qed.
+
+Lemma rinstId'_Tm_pointwise {m_Val : nat} :
+  pointwise_relation _ eq (@ren_Tm m_Val m_Val id) id.
+Proof.
+exact (fun s => eq_ind_r (fun t => t = s) (instId'_Tm s) (rinstInst'_Tm id s)).
+Qed.
+
+Lemma rinstId'_Frame {m_Val : nat} (s : Frame m_Val) : ren_Frame id s = s.
+Proof.
+exact (eq_ind_r (fun t => t = s) (instId'_Frame s) (rinstInst'_Frame id s)).
+Qed.
+
+Lemma rinstId'_Frame_pointwise {m_Val : nat} :
+  pointwise_relation _ eq (@ren_Frame m_Val m_Val id) id.
+Proof.
+exact (fun s =>
+       eq_ind_r (fun t => t = s) (instId'_Frame s) (rinstInst'_Frame id s)).
+Qed.
+
+Lemma varL'_Val {m_Val : nat} {n_Val : nat}
+  (sigma_Val : fin m_Val -> Val n_Val) (x : fin m_Val) :
+  subst_Val sigma_Val (var m_Val x) = sigma_Val x.
+Proof.
+exact (eq_refl).
+Qed.
+
+Lemma varL'_Val_pointwise {m_Val : nat} {n_Val : nat}
+  (sigma_Val : fin m_Val -> Val n_Val) :
+  pointwise_relation _ eq (funcomp (subst_Val sigma_Val) (var m_Val))
+    sigma_Val.
+Proof.
+exact (fun x => eq_refl).
+Qed.
+
+Lemma varLRen'_Val {m_Val : nat} {n_Val : nat}
+  (xi_Val : fin m_Val -> fin n_Val) (x : fin m_Val) :
+  ren_Val xi_Val (var m_Val x) = var n_Val (xi_Val x).
+Proof.
+exact (eq_refl).
+Qed.
+
+Lemma varLRen'_Val_pointwise {m_Val : nat} {n_Val : nat}
+  (xi_Val : fin m_Val -> fin n_Val) :
+  pointwise_relation _ eq (funcomp (ren_Val xi_Val) (var m_Val))
+    (funcomp (var n_Val) xi_Val).
+Proof.
+exact (fun x => eq_refl).
+Qed.
+
+Class Up_Frame X Y :=
+    up_Frame : X -> Y.
+
+Class Up_Tm X Y :=
+    up_Tm : X -> Y.
+
+Class Up_Val X Y :=
+    up_Val : X -> Y.
+
+#[global]
+Instance Subst_Frame  {m_Val n_Val : nat}: (Subst1 _ _ _) :=
+ (@subst_Frame m_Val n_Val).
+
+#[global]
+Instance Subst_Tm  {m_Val n_Val : nat}: (Subst1 _ _ _) :=
+ (@subst_Tm m_Val n_Val).
+
+#[global]
+Instance Subst_Val  {m_Val n_Val : nat}: (Subst1 _ _ _) :=
+ (@subst_Val m_Val n_Val).
+
+#[global]
+Instance Up_Val_Val  {m n_Val : nat}: (Up_Val _ _) := (@up_Val_Val m n_Val).
+
+#[global]
+Instance Ren_Frame  {m_Val n_Val : nat}: (Ren1 _ _ _) :=
+ (@ren_Frame m_Val n_Val).
+
+#[global]
+Instance Ren_Tm  {m_Val n_Val : nat}: (Ren1 _ _ _) := (@ren_Tm m_Val n_Val).
+
+#[global]
+Instance Ren_Val  {m_Val n_Val : nat}: (Ren1 _ _ _) := (@ren_Val m_Val n_Val).
+
+#[global]
+Instance VarInstance_Val  {n_Val : nat}: (Var _ _) := (@var n_Val).
+
+Notation "s [ sigma_Val ]" := (subst_Frame sigma_Val s)
+( at level 7, left associativity, only printing)  : subst_scope.
+
+Notation "↑__Frame" := up_Frame (only printing)  : subst_scope.
+
+Notation "s [ sigma_Val ]" := (subst_Tm sigma_Val s)
+( at level 7, left associativity, only printing)  : subst_scope.
+
+Notation "↑__Tm" := up_Tm (only printing)  : subst_scope.
+
+Notation "s [ sigma_Val ]" := (subst_Val sigma_Val s)
+( at level 7, left associativity, only printing)  : subst_scope.
+
+Notation "↑__Val" := up_Val (only printing)  : subst_scope.
+
+Notation "↑__Val" := up_Val_Val (only printing)  : subst_scope.
+
+Notation "s ⟨ xi_Val ⟩" := (ren_Frame xi_Val s)
+( at level 7, left associativity, only printing)  : subst_scope.
+
+Notation "s ⟨ xi_Val ⟩" := (ren_Tm xi_Val s)
+( at level 7, left associativity, only printing)  : subst_scope.
+
+Notation "s ⟨ xi_Val ⟩" := (ren_Val xi_Val s)
+( at level 7, left associativity, only printing)  : subst_scope.
+
+Notation "'var'" := var ( at level 1, only printing)  : subst_scope.
+
+Notation "x '__Val'" := (@ids _ _ VarInstance_Val x)
+( at level 5, format "x __Val", only printing)  : subst_scope.
+
+Notation "x '__Val'" := (var x) ( at level 5, format "x __Val")  :
+subst_scope.
+
+#[global]
+Instance subst_Frame_morphism  {m_Val : nat} {n_Val : nat}:
+ (Proper (respectful (pointwise_relation _ eq) (respectful eq eq))
+    (@subst_Frame m_Val n_Val)).
+Proof.
+exact (fun f_Val g_Val Eq_Val s t Eq_st =>
+       eq_ind s (fun t' => subst_Frame f_Val s = subst_Frame g_Val t')
+         (ext_Frame f_Val g_Val Eq_Val s) t Eq_st).
+Qed.
+
+#[global]
+Instance subst_Frame_morphism2  {m_Val : nat} {n_Val : nat}:
+ (Proper (respectful (pointwise_relation _ eq) (pointwise_relation _ eq))
+    (@subst_Frame m_Val n_Val)).
+Proof.
+exact (fun f_Val g_Val Eq_Val s => ext_Frame f_Val g_Val Eq_Val s).
+Qed.
+
+#[global]
+Instance subst_Tm_morphism  {m_Val : nat} {n_Val : nat}:
+ (Proper (respectful (pointwise_relation _ eq) (respectful eq eq))
+    (@subst_Tm m_Val n_Val)).
+Proof.
+exact (fun f_Val g_Val Eq_Val s t Eq_st =>
+       eq_ind s (fun t' => subst_Tm f_Val s = subst_Tm g_Val t')
+         (ext_Tm f_Val g_Val Eq_Val s) t Eq_st).
+Qed.
+
+#[global]
+Instance subst_Tm_morphism2  {m_Val : nat} {n_Val : nat}:
+ (Proper (respectful (pointwise_relation _ eq) (pointwise_relation _ eq))
+    (@subst_Tm m_Val n_Val)).
+Proof.
+exact (fun f_Val g_Val Eq_Val s => ext_Tm f_Val g_Val Eq_Val s).
+Qed.
+
+#[global]
+Instance subst_Val_morphism  {m_Val : nat} {n_Val : nat}:
+ (Proper (respectful (pointwise_relation _ eq) (respectful eq eq))
+    (@subst_Val m_Val n_Val)).
+Proof.
+exact (fun f_Val g_Val Eq_Val s t Eq_st =>
+       eq_ind s (fun t' => subst_Val f_Val s = subst_Val g_Val t')
+         (ext_Val f_Val g_Val Eq_Val s) t Eq_st).
+Qed.
+
+#[global]
+Instance subst_Val_morphism2  {m_Val : nat} {n_Val : nat}:
+ (Proper (respectful (pointwise_relation _ eq) (pointwise_relation _ eq))
+    (@subst_Val m_Val n_Val)).
+Proof.
+exact (fun f_Val g_Val Eq_Val s => ext_Val f_Val g_Val Eq_Val s).
+Qed.
+
+#[global]
+Instance ren_Frame_morphism  {m_Val : nat} {n_Val : nat}:
+ (Proper (respectful (pointwise_relation _ eq) (respectful eq eq))
+    (@ren_Frame m_Val n_Val)).
+Proof.
+exact (fun f_Val g_Val Eq_Val s t Eq_st =>
+       eq_ind s (fun t' => ren_Frame f_Val s = ren_Frame g_Val t')
+         (extRen_Frame f_Val g_Val Eq_Val s) t Eq_st).
+Qed.
+
+#[global]
+Instance ren_Frame_morphism2  {m_Val : nat} {n_Val : nat}:
+ (Proper (respectful (pointwise_relation _ eq) (pointwise_relation _ eq))
+    (@ren_Frame m_Val n_Val)).
+Proof.
+exact (fun f_Val g_Val Eq_Val s => extRen_Frame f_Val g_Val Eq_Val s).
+Qed.
+
+#[global]
+Instance ren_Tm_morphism  {m_Val : nat} {n_Val : nat}:
+ (Proper (respectful (pointwise_relation _ eq) (respectful eq eq))
+    (@ren_Tm m_Val n_Val)).
+Proof.
+exact (fun f_Val g_Val Eq_Val s t Eq_st =>
+       eq_ind s (fun t' => ren_Tm f_Val s = ren_Tm g_Val t')
+         (extRen_Tm f_Val g_Val Eq_Val s) t Eq_st).
+Qed.
+
+#[global]
+Instance ren_Tm_morphism2  {m_Val : nat} {n_Val : nat}:
+ (Proper (respectful (pointwise_relation _ eq) (pointwise_relation _ eq))
+    (@ren_Tm m_Val n_Val)).
+Proof.
+exact (fun f_Val g_Val Eq_Val s => extRen_Tm f_Val g_Val Eq_Val s).
+Qed.
+
+#[global]
+Instance ren_Val_morphism  {m_Val : nat} {n_Val : nat}:
+ (Proper (respectful (pointwise_relation _ eq) (respectful eq eq))
+    (@ren_Val m_Val n_Val)).
+Proof.
+exact (fun f_Val g_Val Eq_Val s t Eq_st =>
+       eq_ind s (fun t' => ren_Val f_Val s = ren_Val g_Val t')
+         (extRen_Val f_Val g_Val Eq_Val s) t Eq_st).
+Qed.
+
+#[global]
+Instance ren_Val_morphism2  {m_Val : nat} {n_Val : nat}:
+ (Proper (respectful (pointwise_relation _ eq) (pointwise_relation _ eq))
+    (@ren_Val m_Val n_Val)).
+Proof.
+exact (fun f_Val g_Val Eq_Val s => extRen_Val f_Val g_Val Eq_Val s).
+Qed.
+
+Ltac auto_unfold := repeat
+                     unfold VarInstance_Val, Var, ids, Ren_Val, Ren1, ren1,
+                      Ren_Tm, Ren1, ren1, Ren_Frame, Ren1, ren1, Up_Val_Val,
+                      Up_Val, up_Val, Subst_Val, Subst1, subst1, Subst_Tm,
+                      Subst1, subst1, Subst_Frame, Subst1, subst1.
+
+Tactic Notation "auto_unfold" "in" "*" := repeat
+                                           unfold VarInstance_Val, Var, ids,
+                                            Ren_Val, Ren1, ren1, Ren_Tm,
+                                            Ren1, ren1, Ren_Frame, Ren1,
+                                            ren1, Up_Val_Val, Up_Val, up_Val,
+                                            Subst_Val, Subst1, subst1,
+                                            Subst_Tm, Subst1, subst1,
+                                            Subst_Frame, Subst1, subst1 
+                                            in *.
+
+Ltac asimpl' := repeat (first
+                 [ progress setoid_rewrite substSubst_Frame_pointwise
+                 | progress setoid_rewrite substSubst_Frame
+                 | progress setoid_rewrite substSubst_Tm_pointwise
+                 | progress setoid_rewrite substSubst_Tm
+                 | progress setoid_rewrite substSubst_Val_pointwise
+                 | progress setoid_rewrite substSubst_Val
+                 | progress setoid_rewrite substRen_Frame_pointwise
+                 | progress setoid_rewrite substRen_Frame
+                 | progress setoid_rewrite substRen_Tm_pointwise
+                 | progress setoid_rewrite substRen_Tm
+                 | progress setoid_rewrite substRen_Val_pointwise
+                 | progress setoid_rewrite substRen_Val
+                 | progress setoid_rewrite renSubst_Frame_pointwise
+                 | progress setoid_rewrite renSubst_Frame
+                 | progress setoid_rewrite renSubst_Tm_pointwise
+                 | progress setoid_rewrite renSubst_Tm
+                 | progress setoid_rewrite renSubst_Val_pointwise
+                 | progress setoid_rewrite renSubst_Val
+                 | progress setoid_rewrite renRen'_Frame_pointwise
+                 | progress setoid_rewrite renRen_Frame
+                 | progress setoid_rewrite renRen'_Tm_pointwise
+                 | progress setoid_rewrite renRen_Tm
+                 | progress setoid_rewrite renRen'_Val_pointwise
+                 | progress setoid_rewrite renRen_Val
+                 | progress setoid_rewrite varLRen'_Val_pointwise
+                 | progress setoid_rewrite varLRen'_Val
+                 | progress setoid_rewrite varL'_Val_pointwise
+                 | progress setoid_rewrite varL'_Val
+                 | progress setoid_rewrite rinstId'_Frame_pointwise
+                 | progress setoid_rewrite rinstId'_Frame
+                 | progress setoid_rewrite rinstId'_Tm_pointwise
+                 | progress setoid_rewrite rinstId'_Tm
+                 | progress setoid_rewrite rinstId'_Val_pointwise
+                 | progress setoid_rewrite rinstId'_Val
+                 | progress setoid_rewrite instId'_Frame_pointwise
+                 | progress setoid_rewrite instId'_Frame
+                 | progress setoid_rewrite instId'_Tm_pointwise
+                 | progress setoid_rewrite instId'_Tm
+                 | progress setoid_rewrite instId'_Val_pointwise
+                 | progress setoid_rewrite instId'_Val
+                 | progress
+                    unfold up_list_Val_Val, up_Val_Val, upRen_list_Val_Val,
+                     upRen_Val_Val, up_ren
+                 | progress
+                    cbn[subst_Frame subst_Tm subst_Val ren_Frame ren_Tm
+                       ren_Val]
+                 | progress fsimpl ]).
+
+Ltac asimpl := check_no_evars;
+                repeat
+                 unfold VarInstance_Val, Var, ids, Ren_Val, Ren1, ren1,
+                  Ren_Tm, Ren1, ren1, Ren_Frame, Ren1, ren1, Up_Val_Val,
+                  Up_Val, up_Val, Subst_Val, Subst1, subst1, Subst_Tm,
+                  Subst1, subst1, Subst_Frame, Subst1, subst1 in *;
+                asimpl'; minimize.
+
+Tactic Notation "asimpl" "in" hyp(J) := revert J; asimpl; intros J.
+
+Tactic Notation "auto_case" := auto_case ltac:(asimpl; cbn; eauto).
+
+Ltac substify := auto_unfold; try setoid_rewrite rinstInst'_Frame_pointwise;
+                  try setoid_rewrite rinstInst'_Frame;
+                  try setoid_rewrite rinstInst'_Tm_pointwise;
+                  try setoid_rewrite rinstInst'_Tm;
+                  try setoid_rewrite rinstInst'_Val_pointwise;
+                  try setoid_rewrite rinstInst'_Val.
+
+Ltac renamify := auto_unfold;
+                  try setoid_rewrite_left rinstInst'_Frame_pointwise;
+                  try setoid_rewrite_left rinstInst'_Frame;
+                  try setoid_rewrite_left rinstInst'_Tm_pointwise;
+                  try setoid_rewrite_left rinstInst'_Tm;
+                  try setoid_rewrite_left rinstInst'_Val_pointwise;
+                  try setoid_rewrite_left rinstInst'_Val.
+
+End Core.
+
+Module Extra.
+
+Import
+Core.
+
+Arguments f_handle {n_Val}.
+
+Arguments f_let {n_Val}.
+
+Arguments f_try {n_Val}.
+
+Arguments discontinue {n_Val}.
+
+Arguments exit {n_Val}.
+
+Arguments throw_e {n_Val}.
+
+Arguments continue {n_Val}.
+
+Arguments handle {n_Val}.
+
+Arguments perform {n_Val}.
+
+Arguments letcc {n_Val}.
+
+Arguments throw {n_Val}.
+
+Arguments try {n_Val}.
+
+Arguments raise {n_Val}.
+
+Arguments unfold {n_Val}.
+
+Arguments app {n_Val}.
+
+Arguments case {n_Val}.
+
+Arguments prj {n_Val}.
+
+Arguments ifz {n_Val}.
+
+Arguments let_ {n_Val}.
+
+Arguments ret {n_Val}.
+
+Arguments var {n_Val}.
+
+Arguments v_cons {n_Val}.
+
+Arguments v_nil {n_Val}.
+
+Arguments eff {n_Val}.
+
+Arguments cont {n_Val}.
+
+Arguments fold {n_Val}.
+
+Arguments rec {n_Val}.
+
+Arguments abs {n_Val}.
+
+Arguments inj {n_Val}.
+
+Arguments prod {n_Val}.
+
+Arguments succ {n_Val}.
+
+Arguments zero {n_Val}.
+
+Arguments unit {n_Val}.
+
+#[global] Hint Opaque subst_Frame: rewrite.
+
+#[global] Hint Opaque subst_Tm: rewrite.
+
+#[global] Hint Opaque subst_Val: rewrite.
+
+#[global] Hint Opaque ren_Frame: rewrite.
+
+#[global] Hint Opaque ren_Tm: rewrite.
+
+#[global] Hint Opaque ren_Val: rewrite.
+
+End Extra.
+
+Module interface.
+
+Export Core.
+
+Export Extra.
+
+End interface.
+
+Export interface.
+
