rocq/stlc/small_step.v
@@ -18,7 +18,7 @@ Ltac invert_value_step :=
   end.
 
 Lemma small_step_determinism : 
-  forall e1 e2 , e1 ⤳ e2 -> forall e2', e1 ⤳ e2' -> e2 = e2'.
+  forall e1 e2 , e1 ~> e2 -> forall e2', e1 ~> e2' -> e2 = e2'.
 Proof.
   intros e1 e2 h1.
   induction h1; intros e3 h2; inversion h2; subst.
@@ -35,25 +35,25 @@ Qed.
    For example, recall rule s_app_cong1 of the small-step relation:
 
 
-           e1 ⤳ e1' 
+           e1 ~> e1' 
     -------------------------- :: s_app_cong1
-         e1 e2 ⤳ e1' e2
+         e1 e2 ~> e1' e2
 
    In this module, we define lemma that creates a 
    "virtual rule" of the multi-step relation.
 
-           e1 ⤳* e1' 
+           e1 ~>* e1' 
     -------------------------- :: ms_app_cong1
-       e1 e2 ⤳* e1' e2
+       e1 e2 ~>* e1' e2
 
 *)
 
 (*
 Small.s_app_cong1
-  : forall e1 e1' e2 : Tm 0, e1 ⤳ e1' -> app e1 e2 ⤳ app e1' e2
+  : forall e1 e1' e2 : Tm 0, e1 ~> e1' -> app e1 e2 ~> app e1' e2
 *)
 
-Lemma ms_app_cong1 e1 e1' e2 :  e1 ⤳* e1' ->  app e1 e2 ⤳* app e1' e2.
+Lemma ms_app_cong1 e1 e1' e2 :  e1 ~>* e1' ->  app e1 e2 ~>* app e1' e2.
 Proof.
   induction 1.
   eapply ms_refl.
@@ -65,11 +65,11 @@ Qed.
 
 (*
 Small.s_app_cong2
-  : forall v e2 e2' : Tm 0, is_value v = true -> e2 ⤳ e2' -> app v e2 ⤳ app v e2'
+  : forall v e2 e2' : Tm 0, is_value v = true -> e2 ~> e2' -> app v e2 ~> app v e2'
 *)
 
 Lemma ms_app_cong2 v e2 e2' : 
-  is_value v = true ->  e2 ⤳* e2' ->  app v e2 ⤳* app v e2'.
+  is_value v = true ->  e2 ~>* e2' ->  app v e2 ~>* app v e2'.
 Proof.
   intros h1 h2. 
   induction h2.
